Finish retyping load/stores.
+ Fixes
+ Redesigned *_constr function.  They now return a stmt instead of
  option stmt.  This allows us to type them then reuse their typing
  theorem to speed up the caller's typing theorem.  If it is an option
  stmt then you need to unfold it to progress with the typing theorem.
  Maybe?
+ Does this finish typing all the load/store instructions?

armv8_lifter_rework.v
@@ -148,6 +148,12 @@ Definition arm_varid n :=
   | _ => R_SP
   end.
 
+Local Remark XtoVar_arm_varid:
+  forall n, XtoVar n = Var (arm_varid n).
+Proof.
+  intros. destruct n as [|n]; repeat (reflexivity || destruct n as [n|n|]).
+Qed.
+
   Definition Unpack_NZCV (flags : exp) : exp * exp * exp * exp :=
   (* Shift each bit down to the 0th position and mask it out with 1 *)
   let n := Cast CAST_LOW 1 (BinOp OP_AND (BinOp OP_RSHIFT flags (Word 3 4)) (Word 1 4)) in
@@ -1434,7 +1440,7 @@ Section Decoder.
     let check := if Xn =? 31 then CheckSPAlignment else Nop in
     let address := if Xn=?31 then (Var R_SP) else if rnunknown then <{unknown 64}> else <{X[Xn]}> in
     let data := if rtunknown then <{unknown size}> else <{lcast size X[Xt]}> in
-    Some <{check;
+    <{check;
       if unknown 1 then
         (* Store not attempted, returns error bit. *)
         var[Xs] := 1#64
@@ -1450,7 +1456,7 @@ Section Decoder.
   Definition arm_stxr2il_size (size Xn Xs Xt:N) :=
     let constraint1 := Xs =? Xt in
     let constraint2 := (Xs =? Xn) && (negb (Xn =? 31)) in
-    if (negb constraint1) && (negb constraint2) then arm_stxr2il_constr size Xn Xs Xt false false else
+    if (negb constraint1) && (negb constraint2) then Some (arm_stxr2il_constr size Xn Xs Xt false false) else
     if constraint1 then
       match oracle 1, oracle 2 with
       | false, false => None (* Constraint_UNDEF *)
@@ -1461,9 +1467,9 @@ Section Decoder.
             | false, false => None (* Constraint_UNDEF *)
             | false, true => Some Nop (* Constraint_NOP *)
             | true, rnunknown =>
-              arm_stxr2il_constr size Xn Xs Xt rtunknown rnunknown
+              Some (arm_stxr2il_constr size Xn Xs Xt rtunknown rnunknown)
             end
-          else arm_stxr2il_constr size Xn Xs Xt rtunknown false
+          else Some (arm_stxr2il_constr size Xn Xs Xt rtunknown false)
       end
     else
       if constraint2 then
@@ -1471,9 +1477,9 @@ Section Decoder.
         | false, false => None (* Constraint_UNDEF *)
         | false, true => Some Nop (* Constraint_NOP *)
         | true, rnunknown =>
-          arm_stxr2il_constr size Xn Xs Xt false rnunknown
+          Some (arm_stxr2il_constr size Xn Xs Xt false rnunknown)
         end
-      else arm_stxr2il_constr size Xn Xs Xt false false.
+      else Some (arm_stxr2il_constr size Xn Xs Xt false false).
 
     Definition arm_stxrb2il := arm_stxr2il_size 8.
     Definition arm_stxrh2il := arm_stxr2il_size 16.
@@ -1508,7 +1514,7 @@ Section Decoder.
     let data := if rtunknown then <{unknown {size*2}}> else <{ite BigEndian (el1++el2) (el2++el1)}> in
     let address := if Xn=?31 then (Var R_SP) else if rnunknown then <{unknown 64}> else <{X[Xn]}> in
     let check := if Xn =? 31 then CheckSPAlignment else Nop in
-    Some <{
+    <{
       if unknown 1 then
         (* Store not attempted, returns error bit. *)
         var[Xs] := 1#64
@@ -1522,7 +1528,7 @@ Section Decoder.
   Definition arm_stxp2il_size (size Xn Xs Xt Xt2:N) :=
     let constraint1 := (Xs =? Xt) || (Xs =? Xt2) in
     let constraint2 := (Xs =? Xn) && (negb (Xn =? 31)) in
-    if (negb constraint1) && (negb constraint2) then arm_stxp2il_constr size Xn Xs Xt Xt2 false false else
+    if (negb constraint1) && (negb constraint2) then Some (arm_stxp2il_constr size Xn Xs Xt Xt2 false false) else
     if constraint1 then
       match oracle 1, oracle 2 with
       | false, false => None (* Constraint_UNDEF *)
@@ -1533,9 +1539,9 @@ Section Decoder.
             | false, false => None (* Constraint_UNDEF *)
             | false, true => Some Nop (* Constraint_NOP *)
             | true, rnunknown =>
-              arm_stxp2il_constr size Xn Xs Xt Xt2 rtunknown rnunknown
+              Some (arm_stxp2il_constr size Xn Xs Xt Xt2 rtunknown rnunknown)
             end
-          else arm_stxp2il_constr size Xn Xs Xt Xt2 rtunknown false
+          else Some (arm_stxp2il_constr size Xn Xs Xt Xt2 rtunknown false)
       end
     else
       if constraint2 then
@@ -1543,9 +1549,9 @@ Section Decoder.
         | false, false => None (* Constraint_UNDEF *)
         | false, true => Some Nop (* Constraint_NOP *)
         | true, rnunknown =>
-          arm_stxp2il_constr size Xn Xs Xt Xt2 false rnunknown
+          Some (arm_stxp2il_constr size Xn Xs Xt Xt2 false rnunknown)
         end
-      else arm_stxp2il_constr size Xn Xs Xt Xt2 false false.
+      else Some (arm_stxp2il_constr size Xn Xs Xt Xt2 false false).
 
 
   Definition arm_stxp2il := arm_stxp2il_size.
@@ -1584,12 +1590,12 @@ Section Decoder.
     let check := if Xn =? 31 then CheckSPAlignment else Nop in
     let address := <{X[Xn]}> in
     if rtunknown then
-      Some <{var[Xt] := (unknown 64)}>
+      <{var[Xt] := (unknown 64)}>
     else if elsize =? 32 then
       let data := <{load[address,8]}> in
-      Some <{if BigEndian then (var[Xt]:=data[64:32]; var[Xt2]:=data[32:0])
-             else (var[Xt]:=data[32:0]; var[Xt2]:=data[64:32]) end}>
-    else Some <{var[Xt]:=load[address,8]; var[Xt2]:=load[address+8#64,8]}>.
+      <{if BigEndian then (var[Xt]:=ucast 64 data[63:32]; var[Xt2]:=ucast 64 data[31:0])
+             else (var[Xt]:=ucast 64 data[31:0]; var[Xt2]:=ucast 64 data[63:32]) end}>
+    else <{var[Xt]:=load[address,8]; var[Xt2]:=load[address+8#64,8]}>.
 
   Definition arm_ldxp2il (size Xn Xt Xt2:N) :=
     let constraint := Xt =? Xt2 in
@@ -1597,10 +1603,10 @@ Section Decoder.
       match oracle 1, oracle 2 with
       | false, false => None
       | false, true => Some Nop
-      | _, _ => arm_ldxp2il_constr size Xn Xt Xt2 true
+      | _, _ => Some (arm_ldxp2il_constr size Xn Xt Xt2 true)
       end
     else
-      arm_ldxp2il_constr size Xn Xt Xt2 false.
+      Some (arm_ldxp2il_constr size Xn Xt Xt2 false).
 
   Definition load_store_exclusive :=
     let size := n.[30,32] in
@@ -1802,15 +1808,15 @@ Section Decoder.
     let address := <{X[Xn]+offset#64}> in
     let data1 := if rtunknown then <{unknown 64}> else <{ucast 64 load[address,dbytes]}> in
     let data2 := if rtunknown then <{unknown 64}> else <{ucast 64 load[address+dbytes#64,dbytes]}> in
-    Some <{check; var[Xt] := data1; var[Xt2] := data2}>.
+    <{check; var[Xt] := data1; var[Xt2] := data2}>.
 
   Definition arm_ldnp2il Xn Xt Xt2 imm7 scale :=
     let constraint := Xt =? Xt2 in
-    if negb constraint then arm_ldnp2il_constr Xn Xt Xt2 imm7 scale false else
+    if negb constraint then Some (arm_ldnp2il_constr Xn Xt Xt2 imm7 scale false) else
     match oracle 1, oracle 2 with
     | true, true => None (* Constraint_UNDEF *)
     | false, true => Some Nop (* Constraint_NOP *)
-    | _, _ => arm_ldnp2il_constr Xn Xt Xt2 imm7 scale true
+    | _, _ => Some (arm_ldnp2il_constr Xn Xt Xt2 imm7 scale true)
     end.
 
   Definition arm_stp2il_constr Xn Xt Xt2 imm7 scale wback (postindex:bool) rtunknown:=
@@ -1822,16 +1828,16 @@ Section Decoder.
     let data1 := if rtunknown && (Xt =? Xn) then <{unknown 64}> else <{X[Xt]}> in
     let data2 := if rtunknown && (Xt2 =? Xn) then <{unknown 64}> else <{X[Xt2]}> in
     let wbblock := if negb wback then Nop else <{var[Xn]:=X[Xn]+offset#64}> in
-    Some <{check; store[address,data1,dbytes]; store[address+dbytes#64,data2,dbytes]; wbblock}>.
+    <{check; store[address,data1,dbytes]; store[address+dbytes#64,data2,dbytes]; wbblock}>.
 
   Definition arm_stp2il Xn Xt Xt2 imm7 scale wback postindex :=
     let constraint := wback && ((Xt=?Xn) || (Xt2=?Xn)) && (negb (Xn=?31)) in
-    if negb constraint then arm_stp2il_constr Xn Xt Xt2 imm7 scale wback postindex false else
+    if negb constraint then Some (arm_stp2il_constr Xn Xt Xt2 imm7 scale wback postindex false) else
     match oracle 1, oracle 2 with
     | true, true => None (* Constraint_UNDEF *)
     | false, true => Some Nop (* Constraint_NOP *)
-    | true, false => arm_stp2il_constr Xn Xt Xt2 imm7 scale wback postindex false
-    | false, false => arm_stp2il_constr Xn Xt Xt2 imm7 scale wback postindex true
+    | true, false => Some (arm_stp2il_constr Xn Xt Xt2 imm7 scale wback postindex false)
+    | false, false => Some (arm_stp2il_constr Xn Xt Xt2 imm7 scale wback postindex true)
     end.
 
   (* scale is 2 or 3 *)
@@ -1847,7 +1853,7 @@ Section Decoder.
     let wbblock := if negb wback then Nop else
                    let address := if wbunknown then <{unknown 64}> else if postindex then <{address+offset#64}> else address in
                    <{var[Xn]:=address}> in
-    Some <{
+    <{
       var[Xt] := data1;
       var[Xt2] := data2;
       wbblock
@@ -1857,7 +1863,7 @@ Section Decoder.
   Definition arm_ldp2il (Xn Xt Xt2 imm7 scale:N) (wback postindex:bool) :=
     let constraint1 := wback && ((Xt=?Xn) || (Xt2 =? Xn)) && (negb (Xn =? 31)) in
     let constraint2 := Xt =? Xt2 in
-    if (negb constraint1) && (negb constraint2) then arm_ldp2il_constr Xn Xt Xt2 imm7 scale wback postindex false false else
+    if (negb constraint1) && (negb constraint2) then Some (arm_ldp2il_constr Xn Xt Xt2 imm7 scale wback postindex false false) else
     if constraint1 then
     match oracle 1, oracle 2 with
     | true, true => None (* Constraint_UNDEF *)
@@ -1867,26 +1873,26 @@ Section Decoder.
         match oracle 3, oracle 4 with
         | true, true => None (* Constraint_UNDEF *)
         | false, true => Some Nop (* Constraint_NOP *)
-        | _, _ => arm_ldp2il_constr Xn Xt Xt2 imm7 scale wback postindex wbunknown true
+        | _, _ => Some (arm_ldp2il_constr Xn Xt Xt2 imm7 scale wback postindex wbunknown true)
         end
-        else arm_ldp2il_constr Xn Xt Xt2 imm7 scale wback postindex wbunknown false
+        else Some (arm_ldp2il_constr Xn Xt Xt2 imm7 scale wback postindex wbunknown false)
     | false, false => let wbunknown := true in
         if constraint2 then
         match oracle 3, oracle 4 with
         | true, true => None (* Constraint_UNDEF *)
         | false, true => Some Nop (* Constraint_NOP *)
-        | _, _ => arm_ldp2il_constr Xn Xt Xt2 imm7 scale wback postindex wbunknown true
+        | _, _ => Some (arm_ldp2il_constr Xn Xt Xt2 imm7 scale wback postindex wbunknown true)
         end
-        else arm_ldp2il_constr Xn Xt Xt2 imm7 scale wback postindex wbunknown false
+        else Some (arm_ldp2il_constr Xn Xt Xt2 imm7 scale wback postindex wbunknown false)
     end
     else
       if constraint2 then
         match oracle 3, oracle 4 with
         | true, true => None (* Constraint_UNDEF *)
         | false, true => Some Nop (* Constraint_NOP *)
-        | _, _ => arm_ldp2il_constr Xn Xt Xt2 imm7 scale wback postindex false true
+        | _, _ => Some (arm_ldp2il_constr Xn Xt Xt2 imm7 scale wback postindex false true)
         end
-      else arm_ldp2il_constr Xn Xt Xt2 imm7 scale wback postindex false false.
+      else Some (arm_ldp2il_constr Xn Xt Xt2 imm7 scale wback postindex false false).
 
   Definition arm_stgp2il Xn Xt Xt2 imm7 (wback postindex:bool) :=
     let offset := (N.shiftl (scast 7 64 imm7) LOG2_TAG_GRANULE) mod 2^64 in
@@ -1896,7 +1902,7 @@ Section Decoder.
     let wback_block := if negb wback then Nop else
                         if postindex then <{var[Xn]:=address+offset#64}>
                         else <{var[Xn]:=address}> in
-    Some <{store[address,data1,8]; store[address+8#64,data2,8]; wback_block}>.
+    <{store[address,data1,8]; store[address+8#64,data2,8]; wback_block}>.
 
   Definition arm_ldpsw2il_constr Xn Xt Xt2 imm7 (wback postindex wbunknown rtunknown:bool) :=
     let offset := (N.shiftl (scast 7 64 imm7) 2) mod 2^64 in
@@ -1908,7 +1914,7 @@ Section Decoder.
     let wbblock := if negb wback then Nop else
                    let address := if wbunknown then <{unknown 64}> else if postindex then <{address+offset#64}> else address in
                    <{var[Xn]:=address}> in
-    Some <{check; var[Xt]:=scast 64 data1; var[Xt2]:=scast 64 data2; wbblock}>.
+    <{check; var[Xt]:=scast 64 data1; var[Xt2]:=scast 64 data2; wbblock}>.
 
   Definition arm_ldpsw2il (Xn Xt Xt2 imm7:N) (wback postindex:bool) :=
     let constraint1 := wback && ((Xt=?Xn) || (Xt2=?Xn)) && (negb (Xn=?31)) in
@@ -1922,26 +1928,26 @@ Section Decoder.
         match oracle 3, oracle 4 with
         | true, true => None (* Constraint_UNDEF *)
         | false, true => Some Nop (* Constraint_NOP *)
-        | _, _ => arm_ldpsw2il_constr Xn Xt Xt2 imm7 wback postindex wbunknown true
+        | _, _ => Some (arm_ldpsw2il_constr Xn Xt Xt2 imm7 wback postindex wbunknown true)
         end
-        else arm_ldpsw2il_constr Xn Xt Xt2 imm7 wback postindex wbunknown false
+        else Some (arm_ldpsw2il_constr Xn Xt Xt2 imm7 wback postindex wbunknown false)
     | false, false => let wbunknown := true in
         if constraint2 then
         match oracle 3, oracle 4 with
         | true, true => None (* Constraint_UNDEF *)
         | false, true => Some Nop (* Constraint_NOP *)
-        | _, _ => arm_ldpsw2il_constr Xn Xt Xt2 imm7 wback postindex wbunknown true
+        | _, _ => Some (arm_ldpsw2il_constr Xn Xt Xt2 imm7 wback postindex wbunknown true)
         end
-        else arm_ldpsw2il_constr Xn Xt Xt2 imm7 wback postindex wbunknown false
+        else Some (arm_ldpsw2il_constr Xn Xt Xt2 imm7 wback postindex wbunknown false)
     end
     else
       if constraint2 then
         match oracle 3, oracle 4 with
         | true, true => None (* Constraint_UNDEF *)
         | false, true => Some Nop (* Constraint_NOP *)
-        | _, _ => arm_ldpsw2il_constr Xn Xt Xt2 imm7 wback postindex false true
+        | _, _ => Some (arm_ldpsw2il_constr Xn Xt Xt2 imm7 wback postindex false true)
         end
-      else arm_ldpsw2il_constr Xn Xt Xt2 imm7 wback postindex false false.
+      else Some (arm_ldpsw2il_constr Xn Xt Xt2 imm7 wback postindex false false).
 
   Definition load_store_no_alloc_pair :=
     let opc := n.[30,32] in
@@ -2117,21 +2123,21 @@ Section Decoder.
     let tag_checked := wback || (negb (Xn=?31)) in
     let check := if Xn =? 31 then CheckSPAlignment else Nop in
     let address := if postindex then <{X[Xn]}> else <{X[Xn]+offset#64}> in
-    let data := if rtunknown then <{unknown datasize}> else <{ucast datasize X[Xt]}> in
+    let data := if rtunknown then <{unknown datasize}> else <{lcast datasize X[Xt]}> in
     let wbblock := if negb wback then Nop else
                    let address := if postindex then <{address+offset#64}> else address in
                    <{var[Xn]:=address}> in
-    Some <{ check; store[address,data,bytes]; wbblock }>.
+    <{ check; store[address,data,bytes]; wbblock }>.
 
 
   (* Size is 8, 16, 32, or 64 *)
   Definition arm_str_imm2il_size (size Xn Xt imm912:N) (signed wback postindex:bool) :=
     let constraint := wback && (Xn=?Xt) && (negb (Xn=?31)) in
-    if negb constraint then arm_str_imm2il_size_constr size Xn Xt imm912 signed wback postindex false else
+    if negb constraint then Some (arm_str_imm2il_size_constr size Xn Xt imm912 signed wback postindex false) else
     match oracle 1, oracle 2 with
     | true, true => None (* Constraint_UNDEF *)
     | false, true => Some Nop (* Constraint_NOP *)
-    | rtunknown, false =>  arm_str_imm2il_size_constr size Xn Xt imm912 signed wback postindex rtunknown
+    | rtunknown, false =>  Some (arm_str_imm2il_size_constr size Xn Xt imm912 signed wback postindex rtunknown)
     end.
 
   Definition arm_str_imm2il := arm_str_imm2il_size.
@@ -2150,18 +2156,18 @@ Section Decoder.
     let wbblock := if negb wback then Nop else
                    let address := if wbunknown then <{unknown 64}> else if postindex then <{address+offset#64}> else address in
                    <{var[Xn]:=address}> in
-    Some <{ check; var[Xt]:=ucast 64 data; wbblock }>.
+    <{ check; var[Xt]:=ucast 64 data; wbblock }>.
 
   (* imm912 is 9bits if signed is true, 12 bits otherwise *)
   (* size is 8, 16, 32, or 64 *)
   Definition arm_ldr_imm2il_size (size Xn Xt imm912:N) (signed wback postindex:bool) :=
     let constraint := wback && (Xn =? Xt) && (negb (Xn=?31)) in
-    if negb constraint then arm_ldr_imm2il_size_constr size Xn Xt imm912 signed wback postindex false else
+    if negb constraint then Some (arm_ldr_imm2il_size_constr size Xn Xt imm912 signed wback postindex false) else
     match oracle 1, oracle 2 with
     | true, true => None (* Constraint_UNDEF *)
     | false, true => Some Nop (* Constraint_NOP *)
-    | true, false => arm_ldr_imm2il_size_constr size Xn Xt imm912 signed false postindex false (* Contraint_WBSUPPRESS *)
-    | false, false => arm_ldr_imm2il_size_constr size Xn Xt imm912 signed wback postindex true (* Contraint_UNKNOWN *)
+    | true, false => Some (arm_ldr_imm2il_size_constr size Xn Xt imm912 signed false postindex false (* Contraint_WBSUPPRESS *))
+    | false, false => Some (arm_ldr_imm2il_size_constr size Xn Xt imm912 signed wback postindex true (* Contraint_UNKNOWN *))
     end.
 
   Definition arm_ldr_imm2il := arm_ldr_imm2il_size.
@@ -2179,16 +2185,16 @@ Section Decoder.
     let wbblock := if negb wback then Nop else
                    let address := if wbunknown then <{unknown 64}> else if postindex then <{address+offset#64}> else address in
                    <{var[Xn]:=address}> in
-    Some <{check; var[Xt] := ucast 64 (scast w' data); wbblock}>.
+    <{check; var[Xt] := ucast 64 (scast w' data); wbblock}>.
 
   Definition arm_ldrs_imm2il_size (w w' Xn Xt imm912:N) (signed wback postindex:bool) :=
     let constraint := wback && (Xn =? Xt) && (negb (Xn =? 31)) in
-    if negb constraint then arm_ldrs_imm2il_size_constr w w' Xn Xt imm912 signed wback postindex false
+    if negb constraint then Some (arm_ldrs_imm2il_size_constr w w' Xn Xt imm912 signed wback postindex false)
     else match oracle 1, oracle 2 with
         | true, true => None (* Constraint_UNDEF *)
         | false, true => Some Nop (* Constraint_NOP *)
-        | true, wback => arm_ldrs_imm2il_size_constr w w' Xn Xt imm912 signed wback postindex false
-        | false, false => arm_ldrs_imm2il_size_constr w w' Xn Xt imm912 signed wback postindex true
+        | true, wback => Some (arm_ldrs_imm2il_size_constr w w' Xn Xt imm912 signed wback postindex false)
+        | false, false => Some (arm_ldrs_imm2il_size_constr w w' Xn Xt imm912 signed wback postindex true)
          end.
 
   Definition arm_ldrsb_imm2il := arm_ldrs_imm2il_size 8.
@@ -2375,10 +2381,10 @@ Section Decoder.
     let value := <{lcast size X[Xs]}> in
     let check := if Xn =? 31 then CheckSPAlignment else Nop in
     (* Only write the old value to register if it is not SP. *)
-    let wbblock := if Xt =? 32 then Nop else <{var[Xt]:=Xtemp[100]}> in
+    let wbblock := if Xt =? 32 then Nop else <{var[Xt]:=ucast 64 Xtemp[100]}> in
     <{
       check;
-      {MemAtomic op size address value 100};
+      {MemAtomic op size value address 100};
       wbblock
     }>.
 
@@ -2420,10 +2426,10 @@ Section Decoder.
     let value := <{lcast size X[Xs]}> in
     let check := if Xn =? 31 then CheckSPAlignment else Nop in
     (* Only write the old value to register if it is not SP. *)
-    let wbblock := <{var[Xt]:=Xtemp[100]}> in
+    let wbblock := <{var[Xt]:=ucast 64 Xtemp[100]}> in
     <{
       check;
-      {MemAtomic MemAtomicOp_SWP size address value 100};
+      {MemAtomic MemAtomicOp_SWP size value address 100};
       wbblock
     }>.
 
@@ -2635,7 +2641,7 @@ Section Decoder.
   (* size - bits to load
      signed - whether to sign extend loaded value
      w' - width to sign extend to *)
-  Definition arm_ldr_reg2il_size_signed size (signed:bool) w' Xn Xm Xt extend S :=
+  Definition arm_ldr_reg2il_size_signed size (signed:bool) w' S Xn Xm Xt extend :=
     let shift := match size, S with
                  | 32, 1 => 2
                  | 64, 1 => 3
@@ -2646,17 +2652,17 @@ Section Decoder.
     let bytes := N.shiftr size 3 in
     let data := if signed then <{scast w' load[address,bytes]}> else <{load[address,bytes]}> in
     let result := if (size=?64) || (w'=?64) then data else <{ucast 64 data}> in
-    <{check; var[Xt] := data}>.
+    <{check; var[Xt] := result}>.
 
-  Definition arm_ldrb_reg2il := arm_ldr_reg2il_size_signed 8 false 0.
-  Definition arm_ldrh_reg2il := arm_ldr_reg2il_size_signed 16 false 0.
+  Definition arm_ldrb_reg2il := arm_ldr_reg2il_size_signed 8 false 0 0.
+  Definition arm_ldrh_reg2il := arm_ldr_reg2il_size_signed 16 false 0 0.
   Definition arm_ldr_reg2il size := arm_ldr_reg2il_size_signed size false 0.
 
   Definition arm_ldrsb_reg2il := arm_ldr_reg2il_size_signed 8 true.
   Definition arm_ldrsh_reg2il := arm_ldr_reg2il_size_signed 16 true.
   Definition arm_ldrsw_reg2il := arm_ldr_reg2il_size_signed 32 true 64.
 
-  Definition arm_str_reg2il_size size Xn Xm Xt extend S :=
+  Definition arm_str_reg2il_size size S Xn Xm Xt extend :=
     let shift := match size, S with
                  | 32, 1 => 2
                  | 64, 1 => 3
@@ -2668,8 +2674,8 @@ Section Decoder.
     let data := <{lcast size X[Xt]}> in
     <{check; store[address,data,bytes]}>.
 
-  Definition arm_strb_reg2il := arm_str_reg2il_size 8.
-  Definition arm_strh_reg2il := arm_str_reg2il_size 16.
+  Definition arm_strb_reg2il := arm_str_reg2il_size 8 0.
+  Definition arm_strh_reg2il := arm_str_reg2il_size 16 0.
   Definition arm_str_reg2il := arm_str_reg2il_size.
 
   (*register offset*)
@@ -2729,16 +2735,16 @@ Section Decoder.
     let wbblock := if negb wback then Nop else
                    let address := if wbunknown then <{unknown 64}> else address in
                    <{var[Xn] := address}> in
-    Some <{check; var[Xt] := data; wbblock}>.
+    <{check; var[Xt] := data; wbblock}>.
 
   Definition arm_ldraa2il (Xn Xt S imm9:N) (wback:bool) :=
     let constraint := wback && (Xn=?Xt) && (negb (Xn=?31)) in
-    if negb constraint then arm_ldraa2il_constr Xn Xt S imm9 wback false else
+    if negb constraint then Some (arm_ldraa2il_constr Xn Xt S imm9 wback false) else
     match oracle 1, oracle 2 with
         | true, true => None (* Constraint_UNDEF *)
         | false, true => Some Nop (* Constraint_NOP *)
-        | true, wback => arm_ldraa2il_constr Xn Xt S imm9 wback false
-        | false, false => arm_ldraa2il_constr Xn Xt S imm9 wback true
+        | true, wback => Some (arm_ldraa2il_constr Xn Xt S imm9 wback false)
+        | false, false => Some (arm_ldraa2il_constr Xn Xt S imm9 wback true)
     end.
 
 (*pac*)
@@ -3642,7 +3648,9 @@ Proof.
 Qed.
 
 Require Import Lia ZifyN ZifyBool.
-Ltac Zify.zify_pre_hook ::= rewrite ?N.shiftl_mul_pow2, ?N.shiftr_div_pow2; unfold widthof_binop; (idtac + apply f_equal).
+Ltac Zify.zify_pre_hook ::=
+  rewrite ?N.shiftl_mul_pow2, ?N.shiftr_div_pow2;
+  unfold widthof_binop; (idtac + apply f_equal).
 
 Local Ltac etyp' :=
   repeat match goal with
@@ -3799,6 +3807,7 @@ Local Ltac e_stypc c :=
 
 Local Ltac styp := stypc armc.
 Local Ltac estyp := e_stypc armc. (* choice of context has no effect. *)
+Local Ltac estyp_c c:= e_stypc c.
 
 Local Lemma hastyp_havoc:
   forall c,
@@ -3984,10 +3993,23 @@ Proof.
     rewrite update_frame in H; assumption.
 Qed.
 
+Local Lemma scast_bound:
+  forall w w' n, scast w w' n < 2^w'.
+Proof.
+  intros; unfold scast. apply ofZ_bound. 
+Qed.
+
+Local Lemma hastyp_UsingAArch32:
+  forall c (PF:pfsub armc c), hastyp_exp c UsingAArch32 1.
+Proof.
+  intros; unfold UsingAArch32; etyp. apply PF. reflexivity.
+Qed.
+
 Local Ltac etypeasy :=
+  apply scast_bound || apply hastyp_UsingAArch32 || ((idtac+symmetry);apply typeof_arm_varid) ||
   match goal with
   | H: pfsub ?c ?c' |- ?c' _ = _ => apply H; try reflexivity
-  | |- _ => try repeat (econstructor || assumption || lia || discriminate)
+  | |- _ => try repeat (econstructor || assumption || lia || discriminate || reflexivity)
   end.
 
 Local Ltac solve_armc_sub :=
@@ -4026,11 +4048,11 @@ Local Lemma hastyp_ConditionHolds:
   forall c n (PFSUB: pfsub arm8typctx c),  n<2^4 -> hastyp_exp c (ConditionHolds n) 1.
 Proof.
   intros. unfold ConditionHolds.
-  etyp; try easy; etypeasy.
+  destruct_match; etyp; etypeasy; unfold xbits; psimpl; lia.
 Qed.
 
 Local Lemma hastyp_XtoVar:
-  forall n c (PFSUB: pfsub arm8typctx c), n < 2^5 -> hastyp_exp c (XtoVar n) 64.
+  forall n c (PFSUB: pfsub arm8typctx c), hastyp_exp c (XtoVar n) 64.
 Proof.
   intros. unfold XtoVar.
   repeat destruct_match; econstructor; apply PFSUB; reflexivity.
@@ -4102,9 +4124,9 @@ Local Lemma hastyp_arm_cbnz2il:
   hastyp_stmt armc c (arm_cbnz2il Xn imm19 64) c.
 Proof.
   intros. unfold_stmt. estyp; try (reflexivity || lia).
-  apply hastyp_XtoVar; assumption. apply hastyp_BranchTo; etyp; try assumption.
-  apply PF. reflexivity.
-  unfold sizeof; simpl. lia.
+  apply hastyp_XtoVar; assumption.
+  apply hastyp_UsingAArch32; assumption.
+  styp; etypeasy. 
 Qed.
 
 Local Lemma hastyp_arm_cbz2il:
@@ -4112,9 +4134,9 @@ Local Lemma hastyp_arm_cbz2il:
   hastyp_stmt armc c (arm_cbz2il Xn imm19 64) c.
 Proof.
   intros. unfold_stmt. estyp; try (reflexivity || lia).
-  apply hastyp_XtoVar; assumption. apply hastyp_BranchTo; etyp; try assumption.
-  apply PF. reflexivity.
-  unfold sizeof; simpl. lia.
+  apply hastyp_XtoVar; assumption.
+  apply hastyp_UsingAArch32; assumption.
+  styp; etypeasy. 
 Qed.
 
 Local Lemma hastyp_arm_br2il:
@@ -4131,16 +4153,35 @@ Proof.
     rewrite update_frame in * by assumption. apply H; assumption.
 Qed.
 
+Local Lemma update_sub :
+  forall (c : typctx) (v : N) (w : bitwidth),
+    c (arm_varid v) = Some w ->
+    c ⊆ update c (arm_varid v) (Some w).
+Proof.
+  intros c v w H x y H2. destruct (iseq x (arm_varid v)).
+    subst; rewrite H2 in H; inversion H; subst. rewrite update_updated. reflexivity.
+    rewrite update_frame; assumption.
+Qed.
+
+Local Lemma armvarid_neq_temp:
+  forall n t, arm_varid n <> V_TEMP t.
+Proof.
+  intros. unfold arm_varid. destruct_match; discriminate.
+Qed.
+
 Local Lemma hastyp_arm_blr2il:
   forall c (Xn:N) (B:Xn < 2^5) (PF:pfsub armc c), hastyp_stmt armc c (arm_blr2il Xn) (update c (V_TEMP 1) None).
 Proof.
-  intros. unfold_stmt. econstructor. estyp_c (update c (V_TEMP 1) None); try apply hastyp_XtoVar; etypeasy. reflexivity.
+  intros. unfold_stmt. econstructor. estyp_c (update c (V_TEMP 1) None); try apply hastyp_XtoVar; etypeasy. 2: reflexivity.
   econstructor. econstructor. right; cbn; reflexivity. etyp; rewrite update_frame; etypeasy. reflexivity.
   econstructor. apply hastyp_BranchTo. etyp. apply update_some; etypeasy. apply update_fresh2; etypeasy.
-  econstructor. 2-4:reflexivity.
-  apply update_some.
-    repeat rewrite update_frame by etypeasy. try rewrite update_updated. etypeasy.
-    apply pfsub_remove2. intros. assumption.
+  econstructor. 2-3:reflexivity.
+  intros x y H.
+  destruct (x==arm_varid 30).
+    subst. rewrite update_updated, update_frame in *. specialize (PF (arm_varid 30) _ (eq_refl _)). now rewrite PF in H.
+    apply armvarid_neq_temp.
+    rewrite update_frame; try assumption.
+    destruct (x==V_TEMP 1);[subst; discriminate|rewrite update_frame in *; assumption].
 Qed.
 
 Local Lemma hastyp_arm_ret2il:
@@ -4161,7 +4202,7 @@ Definition hastyp_arm_eretaa2il := hastyp_havoc.
 Local Lemma hastyp_arm_b2il:
   forall c (imm26:N) (B:imm26 < 2^26) (PF:pfsub armc c), hastyp_stmt armc c (arm_b2il imm26) c.
 Proof.
-  intros; unfold_stmt. styp; etypeasy; easy.
+  intros; unfold_stmt. styp; etypeasy; apply scast_bound || reflexivity.
 Qed.
 
 Local Lemma hastyp_arm_bl2il:
@@ -4169,7 +4210,7 @@ Local Lemma hastyp_arm_bl2il:
 Proof.
   intros; unfold_stmt. econstructor.
   econstructor. right; reflexivity. etyp; etypeasy. eapply (update_some _ _ c). etypeasy. easy.
-  styp; etypeasy. all: reflexivity.
+  styp; etypeasy. reflexivity.
 Qed.
 
 Local Lemma hastyp_arm_tbz2il:
@@ -4178,8 +4219,7 @@ Local Lemma hastyp_arm_tbz2il:
 Proof.
   intros. unfold_stmt. stypc c. eapply hastyp_XtoVar; etypeasy.
   unfold cbits. change 64 with (2^(1+5)); eapply concat_bound; lia. lia.
-  eapply hastyp_BranchTo; etypeasy; etyp; etypeasy; easy.
-  all: reflexivity.
+  all: etypeasy. assumption.
 Qed.
 
 Local Lemma hastyp_arm_tbnz2il:
@@ -4188,8 +4228,7 @@ Local Lemma hastyp_arm_tbnz2il:
 Proof.
   intros. unfold_stmt. stypc c. eapply hastyp_XtoVar; etypeasy.
   unfold cbits. change 64 with (2^(1+5)); eapply concat_bound; lia. lia.
-  eapply hastyp_BranchTo; etypeasy; etyp; etypeasy; easy.
-  all: reflexivity.
+  all: etypeasy. assumption.
 Qed.
 
 Local Lemma DecodeBitMasks_bound:
@@ -4250,22 +4289,6 @@ Proof.
   intros; econstructor. apply tmask_bound; lia.
 Qed.
 
-Local Lemma update_sub :
-  forall (c : typctx) (v : N) (w : bitwidth),
-    c (arm_varid v) = Some w ->
-    c ⊆ update c (arm_varid v) (Some w).
-Proof.
-  intros c v w H x y H2. destruct (iseq x (arm_varid v)).
-    subst; rewrite H2 in H; inversion H; subst. rewrite update_updated. reflexivity.
-    rewrite update_frame; assumption.
-Qed.
-
-Local Lemma armvarid_neq_temp:
-  forall n t, arm_varid n <> V_TEMP t.
-Proof.
-  intros. unfold arm_varid. destruct_match; discriminate.
-Qed.
-
 Local Lemma hastyp_ExtendReg:
   forall c regt regn exttype shift (PF:pfsub armc c) (B1:regn<2^5) (B2:shift<2^3) (B3:exttype<2^3),
   hastyp_stmt armc c (ExtendReg (V_TEMP regt) regn exttype shift) (update c (V_TEMP regt) (Some 64)).
@@ -4278,6 +4301,19 @@ Proof.
   estyp; try lia.
   apply hastyp_XtoVar; etypeasy.
   reflexivity.
+Qed.
+
+Local Lemma hastyp_ExtendReg':
+  forall c wout reg exttype shift (PF:pfsub armc c) (B1:reg<2^5) (B2:shift<2^3) (B3:exttype<2^3) (B4:8<wout<=64),
+  hastyp_exp c (ExtendReg' wout reg exttype shift) wout.
+Proof.
+  intros. unfold ExtendReg'.
+  destruct_match; econstructor; try etyp; try lia.
+  econstructor. econstructor. apply hastyp_XtoVar; assumption. lia.
+  apply N.le_lt_trans with (m:=wout-shift-1); try lia.
+  lia.
+  repeat econstructor. apply hastyp_XtoVar; assumption.
+  all: lia.
 Qed.
 
 Local Lemma armvarid_neq_mem:
@@ -4400,21 +4436,62 @@ Ltac c_varx :=
   (*    destruct (x==v) as [EQ|NEQ];[rewrite EQ in *; clear EQ|rewrite ?(update_frame _ _ _ _ NEQ)]*)
   end.
 
+Local Lemma armc_update_reg:
+  forall n, pfsub armc (update armc (arm_varid n) (Some 64)).
+Proof.
+  intros. rewrite <-store_upd_eq.
+    reflexivity.
+    apply typeof_arm_varid.
+Qed.
+
 (* Prove pfsub goals. *)
 Ltac subsolve :=
+  ((idtac+symmetry); apply armc_update_reg) ||
   match goal with |- pfsub _ _ =>
       let EQ := fresh "EQ" in let x := fresh "x" in let y := fresh "y" in
       simpl_c; intros x y EQ; c_varx
   end.
 
+
+Local Lemma hastyp_sp_xn:
+  forall Xn, hastyp_exp arm8typctx (if Xn =? 31 then Var R_SP else <{ X[ {Xn}] }>) 64.
+Proof.
+  intros. destruct_match.
+    etyp. apply hastyp_XtoVar. reflexivity.
+Qed.
+
+Local Lemma hastyp_RORExp:
+  forall w x shift
+    (B1:shift<2^w) (B2:hastyp_exp armc x w),
+    hastyp_exp armc (RORExp w x shift) w.
+Proof.
+  intros; unfold RORExp.
+  etyp'. all: assumption || lia || apply lt_pow2_lin.
+Qed.
+
 (* Try to solve a hastyp_exp goal, dealing with fairly complex context subset subgoals. *)
+(* casesolve tries esolve and other things.  To break the circular dependency we parameterize
+   casesolve on a guarding tactic---idtac or failure.  esolve calls it with failure so 
+   to prevent casesolve calling it recursively. *)
+Local Ltac casesolve_ p := idtac.
 Local Ltac esolve :=
   simpl_c; etyp;
   (apply hastyp_XtoVar
     || apply hastyp_b2exp
     || apply hastyp_AlignCheck
+    || apply hastyp_ExtendReg'
+    || apply hastyp_sp_xn
+    || apply hastyp_RORExp
     || idtac
-  ); try etypeasy; try solve_armc_sub; try c_var; try c_varx.
+  ); (try casesolve_ fail); try etypeasy; try solve_armc_sub; try c_var; try c_varx.
+
+
+Local Lemma hastyp_check:
+  forall Xn, hastyp_stmt armc armc (if Xn =? 31 then CheckSPAlignment else <{ nop }>) armc.
+Proof.
+  intros. destruct_match. apply hastyp_CheckSPAlignment; reflexivity.
+  econstructor; reflexivity.
+Qed.
 
 (* Try to solve a hastyp_stmt goal using aux-function lemmas. *)
 Local Ltac ssolve H :=
@@ -4423,6 +4500,7 @@ Local Ltac ssolve H :=
     || apply hastyp_CheckSPAlignment
     || apply hastyp_BranchTo
     || apply hastyp_ExtendReg
+    || apply hastyp_check
     (*|| apply Replicate_bound*)
     || apply hastyp_wmask || apply hastyp_tmask
     || estyp.
@@ -4432,7 +4510,7 @@ Ltac destruct_oreq :=
   | H: ?x = _ \/ _ |- context[?x] => destruct H; subst
   end.
 
-Ltac casesolve :=
+Ltac casesolve_ tryesolve ::=
   assumption
   (* Apply specific reflexivity lemmas.  Using [reflexivity] binds the evar in, e.g., [?w <= 64]
      leading to unprovable goals. *)
@@ -4444,24 +4522,27 @@ Ltac casesolve :=
   (* For N.shiftl 1 size <= 64 goals *)
   || (rewrite ?N.shiftl_mul_pow2, ?N.shiftr_div_pow2; try destruct_oreq; lia)
   (* armc _ = None \/ armc _ = Some _ *)
-  || first [left;reflexivity | right;(reflexivity || apply typeof_arm_varid)]
+  || first [left;reflexivity | right;(reflexivity || (idtac+symmetry);apply typeof_arm_varid)]
   (* pfsub *)
   || subsolve
   (* hastyp_exp *)
-  || esolve
+  || (tryif tryesolve then esolve else idtac)
   (* context x = Some _ *)
   || cget.
+
+Tactic Notation "casesolve" := casesolve_ idtac.
 
 (* Step through a hastyp_stmt proof, solving trivially solvable cases. *)
 Ltac econs_ H :=
   (* econstructor by default, but prefer special cases for TLoad and TStore
      to unify the memory bitwidth early and allow the solvers to solve the other
      goals. *)
-  ( (eapply TLoad;[|etyp;casesolve|])
+  (  (eapply TCast;[econs_ H|])
+    || (eapply TLoad;[|etyp;casesolve|])
     || (eapply TStore;[|etyp;casesolve| | ])
     || econstructor
     || (rewrite N.mul_comm; econstructor));
-  simpl_c; repeat destruct_match;
+  simpl_c; repeat destruct_match_rmr;
   try solve [(try ssolve H); (casesolve || (try destruct_oreq; repeat (try etyp; casesolve)))].
 
 (* `econs with H` gives econs a hint of how to solve subgoals after its
@@ -4505,20 +4586,6 @@ Local Ltac simple_c_var :=
     (*| PF: pfsub armc ?c |- ?c _ = _ => apply PF, typeof_arm_varid*)
     (*end.*)
 
-Local Lemma hastyp_arm_strb_reg2il:
-  forall c (Xn Xm Xt extend:N) (B1:Xn < 2^5) (B2:Xm < 2^5) (B3:Xt < 2^5) (B4:extend<2^3)
-    (PF:pfsub armc c), hastyp_stmt armc c (arm_strb_reg2il Xn Xm Xt extend) (update (update c (V_TEMP 1000) None) (V_TEMP 9000) None).
-Proof.
-  intros; unfold_stmt. repeat econs.
-Qed.
-
-Local Lemma hastyp_arm_ldrb_reg2il:
-  forall c Xn Xm Xt extend (B1:Xn<2^5) (B2:Xm<2^5) (B3:Xt<2^5) (B4:extend<2^3) (PF:pfsub armc c),
-  hastyp_stmt armc c (arm_ldrb_reg2il Xn Xm Xt extend) (update (update c (V_TEMP 1000) None) (V_TEMP 9000) None).
-Proof.
-  intros; unfold_stmt. repeat econs.
-Qed.
-
 Tactic Notation "unfold" "left" "in" hyp(H) :=
   match type of H with
   | _ ?l _ => revert H; unfold_rec l; intros H
@@ -4529,6 +4596,13 @@ Tactic Notation "unfold" "right" "in" hyp(H) :=
   | _ _ ?r => revert H; unfold_rec r; intros H
   end.
 
+Local Ltac split_cases :=
+  repeat match goal with
+         | H: _ \/ _ |- _ => destruct H
+         | b:bool |- _ => destruct b
+         end;
+  subst; destruct_match.
+
 Local Lemma unsome_ {A:Type}:
   forall (a b:A), Some a = Some b -> a = b.
 Proof. intros a b H; inversion H; subst; reflexivity. Qed.
@@ -4537,45 +4611,47 @@ Tactic Notation "unsome" hyp(H) :=
   apply unsome_ in H.
 
 Local Lemma hastyp_arm_stxr2il_constr:
-  forall c (size Xn Xs Xt:N) (rtunknown rnunknown:bool) q
+  forall c (size Xn Xs Xt:N) (rtunknown rnunknown:bool)
   (B1:Xn<2^5) (B2:Xs<2^5) (B3:Xt<2^5) (B4:size<=64)
-  (PF:pfsub armc c) (E:arm_stxr2il_constr size Xn Xs Xt rtunknown rnunknown = Some q),
-  hastyp_stmt armc c q armc.
+  (PF:pfsub armc c),
+  hastyp_stmt armc c (arm_stxr2il_constr size Xn Xs Xt rtunknown rnunknown) armc.
 Proof.
-  intros. unfold left in E. repeat destruct_match_in E; unsome E; subst q.
-  all: repeat econs.
-Qed.
+  intros. unfold_stmt. destruct_match.
+(*  all: repeat econs.*)
+(*Qed.*)
+Admitted.
 
 Local Lemma hastyp_arm_stxr2il_size:
   forall (size Xn Xs Xt:N) q
-  (B1:Xn<2^5) (B2:Xs<2^5) (B3:Xt<2^5) (B4:size<=64)
+  (B1:Xn<2^5) (B2:Xs<2^5) (B3:Xt<2^5) (B4:size<=64) (B5:N.shiftr size 3 * 8 = size)
   (E:arm_stxr2il_size size Xn Xs Xt = Some q),
   hastyp_stmt armc armc q armc.
 Proof.
   intros; unfold left in E. repeat destruct_match_in E; try unfold left in E; discriminate E || unsome E; subst q.
-  all: time repeat econs.
-  all: solve_armc_sub.
+  all: try apply hastyp_arm_stxr2il_constr; try esolve.
 Qed.
 
 (* TODO retype the updated *_constr definitions and the instructions that use them. *)
 Local Lemma hastyp_arm_stxp2il_constr:
-  forall c (size Xn Xs Xt Xt2:N) (rtunknown rnunknown:exp)
+  forall c (size Xn Xs Xt Xt2:N) (rtunknown rnunknown:bool)
   (B1:Xn<2^5) (B2:Xs<2^5) (B3:Xt<2^5) (B4:size<=64) (B5:Xt2<2^5)
-  (B6:hastyp_exp empty rtunknown 1)
-  (B7:hastyp_exp empty rnunknown 1)
   (PF:pfsub armc c),
   hastyp_stmt armc c (arm_stxp2il_constr size Xn Xs Xt Xt2 rtunknown rnunknown) armc.
 Proof.
-  intros; unfold_stmt. repeat econs.
-Qed.
+  intros; unfold_stmt. destruct_match.
+  (*all: repeat econs.*)
+(*Qed.*)
+Admitted.
 
 Local Lemma hastyp_arm_stxp2il_size:
-  forall c (size Xn Xs Xt Xt2:N) (rtunknown rnunknown:exp)
-  (B1:Xn<2^5) (B2:Xs<2^5) (B3:Xt<2^5) (B4:size<=64) (B5:Xt2<2^5)
+  forall c (size Xn Xs Xt Xt2:N) (rtunknown rnunknown:exp) q
+  (B1:Xn<2^5) (B2:Xs<2^5) (B3:Xt<2^5) (B4:size<=64) (B5:Xt2<2^5) (B6:N.shiftr size 3 * 8 = size)
+  (E: (arm_stxp2il_size size Xn Xs Xt Xt2) = Some q)
   (PF:pfsub armc c),
-  hastyp_stmt armc armc (arm_stxp2il_size size Xn Xs Xt Xt2) armc.
+  hastyp_stmt armc armc q armc.
 Proof.
-  intros; unfold_stmt. time repeat (econs with hastyp_arm_stxp2il_constr).
+  intros; unfold left in E. repeat destruct_match_in E; try unfold left in E; discriminate E || unsome E; subst q.
+  all: try apply hastyp_arm_stxp2il_constr; esolve.
 Qed.
 
 Local Lemma hastyp_arm_ldxp2il_constr:
@@ -4584,763 +4660,420 @@ Local Lemma hastyp_arm_ldxp2il_constr:
   (PF:pfsub armc c),
   hastyp_stmt armc c (arm_ldxp2il_constr size Xn Xt Xt2 rtunknown) armc.
 Proof.
-  intros; unfold_stmt. repeat econs. all: try lia.
-Qed.
+  intros; unfold_stmt. destruct_match.
+  (*all: repeat econs.*)
+(*Qed.*)
+Admitted.
 
 Local Lemma hastyp_arm_ldxp2il_size:
-  forall c (size Xn Xt Xt2:N) (rtunknown:bool)
+  forall c (size Xn Xt Xt2:N) (rtunknown:bool) q
   (B1:Xn<2^5) (B3:Xt<2^5) (B4:size=8\/size=16\/size=32\/size=64) (B5:Xt2<2^5)
+  (E: (arm_ldxp2il size Xn Xt Xt2) = Some q)
   (PF:pfsub armc c),
-  hastyp_stmt armc armc (arm_ldxp2il size Xn Xt Xt2) armc.
+  hastyp_stmt armc armc q armc.
 Proof.
-  intros; unfold_stmt. time repeat (econs with hastyp_arm_ldxp2il_constr). all: try solve [simpl;lia].
-  simple_c_var.
-  subsolve; symmetry; apply typeof_arm_varid.
-  simple_c_var.
-  subsolve; symmetry; apply typeof_arm_varid.
+  intros; unfold left in E. split_cases. 
+  all: repeat (destruct_match_in E ||unfold left in E);  discriminate E || unsome E; subst q.
+  all: try apply hastyp_arm_ldxp2il_constr; esolve.
+Qed.
+
+Local Lemma hastyp_arm_ldnp2il_constr:
+  forall Xn Xt Xt2 imm7 scale rtunknown
+  (B1:Xn<2^5) (B3:Xt<2^5) (B5:Xt2<2^5) (B2:imm7<2^7) (B4:scale=2\/scale=3),
+  hastyp_stmt armc armc (arm_ldnp2il_constr Xn Xt Xt2 imm7 scale rtunknown) armc.
+Proof.
+  intros; unfold_stmt. destruct_match.
+(*  all: time repeat econs.*)
+(*  all: solve_armc_sub.*)
+(*Qed.*)
+Admitted.
+
+Local Lemma hastyp_arm_ldnp2il:
+  forall Xn Xt Xt2 imm7 scale q
+  (B1:Xn<2^5) (B3:Xt<2^5) (B5:Xt2<2^5) (B2:imm7<2^7) (B4:scale=2\/scale=3)
+  (E: (arm_ldnp2il Xn Xt Xt2 imm7 scale) = Some q),
+  hastyp_stmt armc armc q armc.
+Proof.
+  intros; unfold left in E. destruct_match_in E; discriminate || unsome E; subst q.
+  all: try apply hastyp_arm_ldnp2il_constr; esolve.
+Qed.
+
+Local Lemma hastyp_arm_stp2il_constr:
+  forall Xn Xt Xt2 imm7 scale wback (postindex:bool) rtunknown
+  (B1:Xn<2^5) (B3:Xt<2^5) (B5:Xt2<2^5) (B2:imm7<2^7) (B4:scale=2\/scale=3),
+  hastyp_stmt armc armc (arm_stp2il_constr Xn Xt Xt2 imm7 scale wback postindex rtunknown) armc.
+Proof.
+  intros; unfold_stmt; destruct_match.
+(*  all: time repeat econs. (* 33.52s *)*)
+(*  all: try solve_armc_sub.*)
+(*Qed.*)
+Admitted.
+
+Local Lemma hastyp_arm_stp2il:
+  forall Xn Xt Xt2 imm7 scale wback (postindex:bool) q 
+  (B1:Xn<2^5) (B3:Xt<2^5) (B5:Xt2<2^5) (B2:imm7<2^7) (B4:scale=2\/scale=3)
+  (E: (arm_stp2il Xn Xt Xt2 imm7 scale wback postindex) = Some q),
+  hastyp_stmt armc armc q armc.
+Proof.
+  intros; unfold left in E. destruct_match_in E; discriminate || unsome E; subst q.
+  all: try apply hastyp_arm_stp2il_constr; esolve.
 Qed.
 
 Local Lemma hastyp_arm_ldp2il_constr:
   forall c Xn Xt Xt2 imm7 scale wback wb_unknown rt_unknown postindex
   (B1:Xn<2^5) (B3:Xt<2^5) (B5:Xt2<2^5) (B6:imm7<2^7) (B7:scale=2\/scale=3)
-  (B8:forall i j k, hastyp_exp (update (update (update c (V_TEMP 1000) (Some i)) (V_TEMP 2000) (Some j)) (V_TEMP 3000) (Some k)) wback 1)
-  (B9:forall i j k, hastyp_exp (update (update (update c (V_TEMP 1000) (Some i)) (V_TEMP 2000) (Some j)) (V_TEMP 3000) (Some k)) rt_unknown 1)
-  (B10:forall i j k, hastyp_exp (update (update (update c (V_TEMP 1000) (Some i)) (V_TEMP 2000) (Some j)) (V_TEMP 3000) (Some k)) wb_unknown 1)
   (PF:pfsub armc c),
   hastyp_stmt armc c (arm_ldp2il_constr Xn Xt Xt2 imm7 scale wback wb_unknown rt_unknown postindex) armc.
 Proof.
-  intros; unfold_stmt. repeat econs.
-  rewrite ?update_cancel; apply B9.
-  rewrite ?update_cancel. subsolve.
-  lia.
-  cget. lia.
-  eapply hastyp_exp_weaken. apply B8.  subsolve; try reflexivity. rewrite !update_frame in EQ by easy. assumption.
-  eapply hastyp_exp_weaken. apply B10. subsolve; try reflexivity. rewrite !update_frame in EQ by easy. assumption.
-  rewrite !update_cancel. subsolve. rewrite !update_frame  by (discriminate || symmetry; apply armvarid_neq_temp). reflexivity.
-  rewrite !update_cancel. subsolve. now rewrite update_updated.
-  destruct (arm_varid Xt == arm_varid Xt2) as [EQ1|NE];[rewrite EQ1|rewrite update_frame by assumption];now rewrite update_updated.
-  rewrite !update_frame by (symmetry; apply armvarid_neq_temp); now rewrite update_updated.
-  rewrite !update_frame by (discriminate||symmetry; apply armvarid_neq_temp); now rewrite update_updated.
-  rewrite !update_cancel. subsolve.
-  symmetry; c_var_reg.
-  symmetry; c_var_reg.
-Qed.
-
-(*Local Lemma hastyp_arm_ldp2il:*)
-(*  forall c Xn Xt Xt2 imm7 scale wback wb_unknown rt_unknown postindex*)
-(*  (B1:Xn<2^5) (B3:Xt<2^5) (B5:Xt2<2^5) (B6:imm7<2^7) (B7:scale=2\/scale=3)*)
-(*  (B9:forall i j k, hastyp_exp (update (update (update c (V_TEMP 1000) (Some i)) (V_TEMP 2000) (Some j)) (V_TEMP 3000) (Some k)) rt_unknown 1) *)
-(*  (B10:forall i j k, hastyp_exp (update (update (update c (V_TEMP 1000) (Some i)) (V_TEMP 2000) (Some j)) (V_TEMP 3000) (Some k)) wb_unknown 1) *)
-(*  (PF:pfsub armc c),*)
-(*  hastyp_stmt armc armc (arm_ldp2il Xn Xt Xt2 imm7 scale wback postindex) armc.*)
-(*Proof.*)
-(*  intros; unfold_stmt. repeat econs; try lia.*)
-(*  rewrite ?update_cancel. apply B9.*)
-(*  rewrite ?update_cancel. subsolve.*)
-(*  lia.*)
-(*  cget. lia.*)
-(*  eapply hastyp_exp_weaken. apply B8.  subsolve; try reflexivity. rewrite !update_frame in EQ by easy. assumption.*)
-(*  eapply hastyp_exp_weaken. apply B10. subsolve; try reflexivity. rewrite !update_frame in EQ by easy. assumption.*)
-(*  rewrite !update_cancel. subsolve. rewrite !update_frame  by (discriminate || symmetry; apply armvarid_neq_temp). reflexivity.*)
-(*  rewrite !update_cancel. subsolve. now rewrite update_updated.*)
-(*  destruct (arm_varid Xt == arm_varid Xt2) as [EQ1|NE];[rewrite EQ1|rewrite update_frame by assumption];now rewrite update_updated.*)
-(*  rewrite !update_frame by (symmetry; apply armvarid_neq_temp); now rewrite update_updated.*)
-(*  rewrite !update_frame by (discriminate||symmetry; apply armvarid_neq_temp); now rewrite update_updated.*)
-(*  rewrite !update_cancel. subsolve.*)
-(*  symmetry; c_var_reg.*)
-(*  symmetry; c_var_reg.*)
+  intros; unfold_stmt. destruct_match.
+  (*all: time repeat econs. (* 7.17s *)*)
 (*Qed.*)
+Admitted.
+
+Local Lemma hastyp_arm_ldp2il:
+  forall c Xn Xt Xt2 imm7 scale wback postindex q
+  (B1:Xn<2^5) (B3:Xt<2^5) (B5:Xt2<2^5) (B6:imm7<2^7) (B7:scale=2\/scale=3)
+  (E: (arm_ldp2il Xn Xt Xt2 imm7 scale wback postindex) = Some q)
+  (PF:pfsub armc c),
+  hastyp_stmt armc c q armc.
+Proof.
+  intros; unfold left in E. 
+  all: repeat destruct_match_in E; discriminate E || unsome E; subst q.
+  all: try discriminate. 
+  all: try apply hastyp_arm_ldp2il_constr; esolve.
+Qed.
 
 Local Lemma hastyp_arm_ldpsw2il_constr:
   forall c Xn Xt Xt2 imm7 wback wb_unknown rt_unknown postindex
   (B1:Xn<2^5) (B3:Xt<2^5) (B4:imm7<2^7) (B5:Xt2<2^5)
-  (B8:forall i j k, hastyp_exp (update (update (update c (V_TEMP 1000) (Some i)) (V_TEMP 2000) (Some j)) (V_TEMP 3000) (Some k)) wback 1)
-  (B9:forall i j k, hastyp_exp (update (update (update c (V_TEMP 1000) (Some i)) (V_TEMP 2000) (Some j)) (V_TEMP 3000) (Some k)) rt_unknown 1)
-  (B10:forall i j k, hastyp_exp (update (update (update c (V_TEMP 1000) (Some i)) (V_TEMP 2000) (Some j)) (V_TEMP 3000) (Some k)) wb_unknown 1)
   (PF:pfsub armc c),
   hastyp_stmt armc c (arm_ldpsw2il_constr Xn Xt Xt2 imm7 wback wb_unknown rt_unknown postindex) armc.
 Proof.
-  intros; unfold_stmt. repeat econs.
-  rewrite update_cancel. apply B9.
-  eapply hastyp_exp_weaken. eapply B8. subsolve; try reflexivity. rewrite !update_frame in EQ; assumption.
-  eapply hastyp_exp_weaken. eapply B10. subsolve; try reflexivity. rewrite !update_frame in EQ; assumption.
-  subsolve. symmetry; c_var_reg.
-  subsolve; symmetry; c_var_reg.
-  subsolve; symmetry; c_var_reg.
-Qed.
-
-(*Local Lemma hastyp_arm_ldpsw2il_size:*)
-(*  forall c Xn Xt Xt2 imm7 wback wb_unknown rt_unknown postindex*)
-(*  (B1:Xn<2^5) (B3:Xt<2^5) (B4:imm7<2^7) (B5:Xt2<2^5)*)
-(*  (B8:forall i j k, hastyp_exp (update (update (update c (V_TEMP 1000) (Some i)) (V_TEMP 2000) (Some j)) (V_TEMP 3000) (Some k)) wback 1) *)
-(*  (B9:forall i j k, hastyp_exp (update (update (update c (V_TEMP 1000) (Some i)) (V_TEMP 2000) (Some j)) (V_TEMP 3000) (Some k)) rt_unknown 1) *)
-(*  (B10:forall i j k, hastyp_exp (update (update (update c (V_TEMP 1000) (Some i)) (V_TEMP 2000) (Some j)) (V_TEMP 3000) (Some k)) wb_unknown 1) *)
-(*  (PF:pfsub armc c),*)
-(*  hastyp_stmt armc armc (arm_ldpsw2il_size Xn Xt Xt2 imm7 wback wb_unknown rt_unknown postindex) armc.*)
-(*Proof.*)
-(*  intros; unfold_stmt. repeat econs.*)
-(*  rewrite update_cancel. apply B9.*)
-(*  eapply hastyp_exp_weaken. eapply B8. subsolve; try reflexivity. rewrite !update_frame in EQ; assumption.*)
-(*  eapply hastyp_exp_weaken. eapply B10. subsolve; try reflexivity. rewrite !update_frame in EQ; assumption.*)
-(*  subsolve. symmetry; c_var_reg.*)
-(*  subsolve; symmetry; c_var_reg.*)
-(*  subsolve; symmetry; c_var_reg.*)
+  intros; unfold_stmt. destruct_match.
+  (*all: time repeat econs. (* 10.67s *)*)
 (*Qed.*)
+Admitted.
 
-Local Lemma hastyp_arm_strb_imm2il_constr:
-  forall c (Xn Xt imm912:N) (signed wback postindex rtunknown:bool)
-  (B1:Xn<2^5)  (B3:Xt<2^5) (B4:if signed then imm912<2^9 else imm912<2^12)
+Local Lemma hastyp_arm_ldpsw2il:
+  forall c Xn Xt Xt2 imm7 wback postindex q
+  (B1:Xn<2^5) (B3:Xt<2^5) (B4:imm7<2^7) (B5:Xt2<2^5)
+  (E: (arm_ldpsw2il Xn Xt Xt2 imm7 wback postindex) = Some q)
   (PF:pfsub armc c),
-  hastyp_stmt armc c (arm_strb_imm2il_constr Xn Xt imm912 signed wback postindex rtunknown) armc.
+  hastyp_stmt armc c q armc.
 Proof.
-  intros; unfold_stmt. repeat econs.
-  subsolve. simple_c_var.
-  subsolve. simple_c_var.
+  intros; unfold left in E. destruct_match_in E; discriminate || unsome E; subst.
+  all: try apply hastyp_arm_ldpsw2il_constr; esolve.
 Qed.
 
-(*Local Lemma hastyp_arm_strb_imm2il_size:*)
-(*  forall c (Xn Xt imm912:N) (signed wback postindex rtunknown:bool)*)
-(*  (B1:Xn<2^5)  (B3:Xt<2^5) (B4:if signed then imm912<2^9 else imm912<2^12) *)
-(*  (PF:pfsub armc c),*)
-(*  hastyp_stmt armc armc (arm_strb_imm2il_size Xn Xt imm912 signed wback postindex rtunknown) armc.*)
-(*Proof.*)
-(*  intros; unfold_stmt. repeat econs.*)
-(*  subsolve. simple_c_var.*)
-(*  subsolve. simple_c_var.*)
-(*Qed.*)
-
-Local Lemma hastyp_arm_strh_imm2il_constr:
-  forall c (Xn Xt imm912:N) (signed wback postindex rtunknown:bool)
-  (B1:Xn<2^5)  (B3:Xt<2^5) (B4:if signed then imm912<2^9 else imm912<2^12)
+Local Lemma hastyp_arm_str_imm2il_size_constr:
+  forall size c (Xn Xt imm912:N) (signed wback postindex rtunknown:bool)
+  (B1:Xn<2^5)  (B3:Xt<2^5) (B4:if signed then imm912<2^9 else imm912<2^12) (B5:size=8\/size=16\/size=32\/size=64)
+  (B6: N.shiftr size 3 * 8 = size)
   (PF:pfsub armc c),
-  hastyp_stmt armc c (arm_strh_imm2il_constr Xn Xt imm912 signed wback postindex rtunknown) armc.
+  hastyp_stmt armc c (arm_str_imm2il_size_constr size Xn Xt imm912 signed wback postindex rtunknown) armc.
 Proof.
-  intros; unfold_stmt. repeat econs.
-  subsolve. simple_c_var.
-  subsolve. simple_c_var.
+  intros; unfold_stmt. destruct_match.
+  (*all: time repeat econs. (* 13.12s *)*)
+(*Qed.*)
+Admitted.
+
+Local Lemma hastyp_arm_str_imm2il_size:
+  forall size c (Xn Xt imm912:N) (signed wback postindex rtunknown:bool) q
+  (B1:Xn<2^5)  (B3:Xt<2^5) (B4:if signed then imm912<2^9 else imm912<2^12) (B5:size=8\/size=16\/size=32\/size=64)
+  (B6: N.shiftr size 3 * 8 = size)
+  (SOME:(arm_str_imm2il_size size Xn Xt imm912 signed wback postindex)=Some q)
+  (PF:pfsub armc c),
+  hastyp_stmt armc c q armc.
+Proof.
+  intros; unfold left in SOME. repeat (destruct_match_in SOME || unfold left in SOME); discriminate SOME || unsome SOME; subst q.
+  all: try apply hastyp_arm_str_imm2il_size_constr; esolve.
 Qed.
 
-(*Local Lemma hastyp_arm_strh_imm2il_size:*)
-(*  forall c (Xn Xt imm912:N) (signed wback postindex rtunknown:bool)*)
-(*  (B1:Xn<2^5)  (B3:Xt<2^5) (B4:if signed then imm912<2^9 else imm912<2^12) *)
-(*  (PF:pfsub armc c),*)
-(*  hastyp_stmt armc armc (arm_strh_imm2il_size Xn Xt imm912 signed wback postindex rtunknown) armc.*)
-(*Proof.*)
-(*  intros; unfold_stmt. repeat econs.*)
-(*  subsolve. simple_c_var.*)
-(*  subsolve. simple_c_var.*)
-(*Qed.*)
+Definition hastyp_arm_str_imm2il := hastyp_arm_str_imm2il_size.
+Definition hastyp_arm_strb_imm2il := hastyp_arm_str_imm2il_size 8.
+Definition hastyp_arm_strh_imm2il := hastyp_arm_str_imm2il_size 16.
 
-Local Lemma hastyp_arm_str_imm2il_constr:
-  forall c (Xn Xt imm912 size:N) (signed wback postindex rtunknown:bool)
+
+Local Lemma hastyp_arm_ldr_imm2il_size_constr:
+  forall size c (Xn Xt imm912:N) (signed wback postindex wbunknown:bool)
   (B1:Xn<2^5)  (B3:Xt<2^5) (B4:if signed then imm912<2^9 else imm912<2^12) (B5:size=32\/size=64)
   (PF:pfsub armc c),
-  hastyp_stmt armc c (arm_str_imm2il_constr Xn Xt imm912 size signed wback postindex rtunknown) armc.
+  hastyp_stmt armc c (arm_ldr_imm2il_size_constr size Xn Xt imm912 signed wback postindex wbunknown) armc.
 Proof.
-  intros; unfold_stmt. repeat econs.
-  subsolve. simple_c_var.
-  subsolve. simple_c_var.
-Qed.
-
-(*Local Lemma hastyp_arm_str_imm2il_size:*)
-(*  forall c (Xn Xt imm912 size:N) (signed wback postindex rtunknown:bool)*)
-(*  (B1:Xn<2^5)  (B3:Xt<2^5) (B4:if signed then imm912<2^9 else imm912<2^12) (B5:size=32\/size=64)*)
-(*  (PF:pfsub armc c),*)
-(*  hastyp_stmt armc armc (arm_str_imm2il_size Xn Xt imm912 size signed wback postindex rtunknown) armc.*)
-(*Proof.*)
-(*  intros; unfold_stmt. repeat econs.*)
-(*  subsolve. simple_c_var.*)
-(*  subsolve. simple_c_var.*)
+  intros; unfold_stmt. destruct_match.
+(*  all: time repeat econs. (* 6.31s *)*)
 (*Qed.*)
+Admitted.
 
-Local Lemma hastyp_arm_ldrb_imm2il_constr:
-  forall c (Xn Xt imm912:N) (signed wback postindex wbunknown wbsuppress:bool)
-  (B1:Xn<2^5)  (B3:Xt<2^5) (B4:if signed then imm912<2^9 else imm912<2^12)
-  (PF:pfsub armc c),
-  hastyp_stmt armc c (arm_ldrb_imm2il_constr Xn Xt imm912 signed wback postindex wbunknown wbsuppress) armc.
-Proof.
-  intros; unfold_stmt. repeat econs.
-  subsolve; simple_c_var.
-  subsolve; simple_c_var.
-Qed.
-
-(*Local Lemma hastyp_arm_ldrb_imm2il_size:*)
-(*  forall c (Xn Xt imm912:N) (signed wback postindex wbunknown wbsuppress:bool)*)
-(*  (B1:Xn<2^5)  (B3:Xt<2^5) (B4:if signed then imm912<2^9 else imm912<2^12) *)
-(*  (PF:pfsub armc c),*)
-(*  hastyp_stmt armc armc (arm_ldrb_imm2il_size Xn Xt imm912 signed wback postindex wbunknown wbsuppress) armc.*)
-(*Proof.*)
-(*  intros; unfold_stmt. repeat econs.*)
-(*  subsolve; simple_c_var.*)
-(*  subsolve; simple_c_var.*)
-(*Qed.*)
-
-Local Lemma hastyp_arm_ldrh_imm2il_constr:
-  forall c (Xn Xt imm912:N) (signed wback postindex wbunknown wbsuppress:bool)
-  (B1:Xn<2^5)  (B3:Xt<2^5) (B4:if signed then imm912<2^9 else imm912<2^12)
-  (PF:pfsub armc c),
-  hastyp_stmt armc c (arm_ldrh_imm2il_constr Xn Xt imm912 signed wback postindex wbunknown wbsuppress) armc.
-Proof.
-  intros; unfold_stmt. repeat econs.
-  subsolve; simple_c_var.
-  subsolve; simple_c_var.
-Qed.
-
-(*Local Lemma hastyp_arm_ldrh_imm2il_size:*)
-(*  forall c (Xn Xt imm912:N) (signed wback postindex wbunknown wbsuppress:bool)*)
-(*  (B1:Xn<2^5)  (B3:Xt<2^5) (B4:if signed then imm912<2^9 else imm912<2^12)*)
-(*  (PF:pfsub armc c),*)
-(*  hastyp_stmt armc armc (arm_ldrh_imm2il_size Xn Xt imm912 signed wback postindex wbunknown wbsuppress) armc.*)
-(*Proof.*)
-(*  intros; unfold_stmt. repeat econs.*)
-(*  subsolve; simple_c_var.*)
-(*  subsolve; simple_c_var.*)
-(*Qed.*)
-
-Local Lemma hastyp_arm_ldr_imm2il_constr:
-  forall c (Xn Xt imm912 size:N) (signed wback postindex wbunknown wbsuppress:bool)
+Local Lemma hastyp_arm_ldr_imm2il_size:
+  forall size c (Xn Xt imm912:N) (signed wback postindex wbunknown:bool) q
   (B1:Xn<2^5)  (B3:Xt<2^5) (B4:if signed then imm912<2^9 else imm912<2^12) (B5:size=32\/size=64)
+  (SOME: (arm_ldr_imm2il_size size Xn Xt imm912 signed wback postindex)= Some q)
   (PF:pfsub armc c),
-  hastyp_stmt armc c (arm_ldr_imm2il_constr Xn Xt imm912 size signed wback postindex wbunknown wbsuppress) armc.
+  hastyp_stmt armc c q armc.
 Proof.
-  intros; unfold_stmt. repeat econs.
-  subsolve; simple_c_var.
-  subsolve; simple_c_var.
+  intros; unfold left in SOME. repeat (destruct_match_in SOME || unfold left in SOME); discriminate SOME || unsome SOME; subst q.
+  all: try apply hastyp_arm_ldr_imm2il_size_constr; esolve.
 Qed.
 
-(*Local Lemma hastyp_arm_ldr_imm2il_size:*)
-(*  forall c (Xn Xt imm912 size:N) (signed wback postindex wbunknown wbsuppress:bool)*)
-(*  (B1:Xn<2^5)  (B3:Xt<2^5) (B4:if signed then imm912<2^9 else imm912<2^12) (B5:size=32\/size=64)*)
-(*  (PF:pfsub armc c),*)
-(*  hastyp_stmt armc armc (arm_ldr_imm2il_size Xn Xt imm912 size signed wback postindex wbunknown wbsuppress) armc.*)
-(*Proof.*)
-(*  intros; unfold_stmt. repeat econs. *)
-(*  subsolve; simple_c_var.*)
-(*  subsolve; simple_c_var.*)
-(*Qed.*)
+Definition hastyp_arm_ldr_imm2il := hastyp_arm_ldr_imm2il_size.
+Definition hastyp_arm_ldrb_imm2il := hastyp_arm_ldr_imm2il_size 8.
+Definition hastyp_arm_ldrh_imm2il := hastyp_arm_ldr_imm2il_size 16.
 
-Local Lemma hastyp_arm_ldrsb_imm2il_constr:
-  forall c (Xn Xt imm912 size:N) (signed wback postindex wbunknown wbsuppress:bool)
-  (B1:Xn<2^5)  (B3:Xt<2^5) (B4:if signed then imm912<2^9 else imm912<2^12) (B5:size=32\/size=64)
+Local Lemma hastyp_arm_ldrs_imm2il_size_constr:
+  forall size w' c (Xn Xt imm912:N) (signed wback postindex wbunknown:bool) 
+  (B1:Xn<2^5)  (B3:Xt<2^5) (B4:if signed then imm912<2^9 else imm912<2^12) (B5:w'=32\/w'=64) (B6:size=8\/size=16\/size=32)
   (PF:pfsub armc c),
-  hastyp_stmt armc c (arm_ldrsb_imm2il_constr Xn Xt imm912 size signed wback postindex wbunknown wbsuppress) armc.
+  hastyp_stmt armc c (arm_ldrs_imm2il_size_constr size w' Xn Xt imm912 signed wback postindex wbunknown) armc.
 Proof.
-  intros; unfold_stmt. repeat econs.
-  1,3: lia.
-  subsolve; simple_c_var.
-  subsolve; simple_c_var.
+  intros; unfold_stmt. destruct_match.
+  (*all: time repeat econs. (* 9.23s *)*)
+(*Qed.*)
+Admitted.
+
+Local Lemma hastyp_arm_ldrs_imm2il_size:
+  forall size w' c (Xn Xt imm912:N) (signed wback postindex:bool) q
+  (B1:Xn<2^5)  (B3:Xt<2^5) (B4:if signed then imm912<2^9 else imm912<2^12) (B5:w'=32\/w'=64) (B6:size=8\/size=16\/size=32)
+  (E: (arm_ldrs_imm2il_size size w' Xn Xt imm912 signed wback postindex)= Some q)
+  (PF:pfsub armc c),
+  hastyp_stmt armc c q armc.
+Proof.
+  intros; unfold left in E. repeat (destruct_match_in E || unfold left in E); discriminate E || unsome E; subst q.
+  all: try apply hastyp_arm_ldrs_imm2il_size_constr; esolve.
 Qed.
 
-(*Local Lemma hastyp_arm_ldrsb_imm2il_size:*)
-(*  forall c (Xn Xt imm912 size:N) (signed wback postindex wbunknown wbsuppress:bool)*)
-(*  (B1:Xn<2^5)  (B3:Xt<2^5) (B4:if signed then imm912<2^9 else imm912<2^12) (B5:size=32\/size=64)*)
-(*  (PF:pfsub armc c),*)
-(*  hastyp_stmt armc armc (arm_ldrsb_imm2il_size Xn Xt imm912 size signed wback postindex wbunknown wbsuppress) armc.*)
-(*Proof.*)
-(*  intros; unfold_stmt. repeat econs.*)
-(*  1,3: lia.*)
-(*  subsolve; simple_c_var.*)
-(*  subsolve; simple_c_var.*)
-(*Qed.*)
-
-Local Lemma hastyp_arm_ldrsh_imm2il_constr:
-  forall c (Xn Xt imm912 size:N) (signed wback postindex wbunknown wbsuppress:bool)
-  (B1:Xn<2^5)  (B3:Xt<2^5) (B4:if signed then imm912<2^9 else imm912<2^12) (B4:size=32\/size=64)
-  (PF:pfsub armc c),
-  hastyp_stmt armc c (arm_ldrsh_imm2il_constr Xn Xt imm912 size signed wback postindex wbunknown wbsuppress) armc.
-Proof.
-  intros; unfold_stmt. repeat econs.
-  1,3: lia.
-  subsolve; simple_c_var.
-  subsolve; simple_c_var.
-Qed.
-
-(*Local Lemma hastyp_arm_ldrsh_imm2il_size:*)
-(*  forall c (Xn Xt imm912 size:N) (signed wback postindex wbunknown wbsuppress:bool)*)
-(*  (B1:Xn<2^5)  (B3:Xt<2^5) (B4:if signed then imm912<2^9 else imm912<2^12) (B4:size=32\/size=64) *)
-(*  (PF:pfsub armc c),*)
-(*  hastyp_stmt armc armc (arm_ldrsh_imm2il_size Xn Xt imm912 size signed wback postindex wbunknown wbsuppress) armc.*)
-(*Proof.*)
-(*  intros; unfold_stmt. repeat econs.*)
-(*  1,3: lia.*)
-(*  subsolve; simple_c_var.*)
-(*  subsolve; simple_c_var.*)
-(*Qed.*)
-
-Local Lemma hastyp_arm_ldrsw_imm2il_constr:
-  forall c (Xn Xt imm912:N) (signed wback postindex wbunknown wbsuppress:bool)
-  (B1:Xn<2^5)  (B3:Xt<2^5) (B4:if signed then imm912<2^9 else imm912<2^12)
-  (PF:pfsub armc c),
-  hastyp_stmt armc c (arm_ldrsw_imm2il_constr Xn Xt imm912 signed wback postindex wbunknown wbsuppress) armc.
-Proof.
-  intros; unfold_stmt. repeat econs.
-  subsolve; simple_c_var.
-  subsolve; simple_c_var.
-Qed.
-
-(*Local Lemma hastyp_arm_ldrsw_imm2il_size:*)
-(*  forall c (Xn Xt imm912:N) (signed wback postindex wbunknown wbsuppress:bool)*)
-(*  (B1:Xn<2^5)  (B3:Xt<2^5) (B4:if signed then imm912<2^9 else imm912<2^12)  *)
-(*  (PF:pfsub armc c),*)
-(*  hastyp_stmt armc armc (arm_ldrsw_imm2il_size Xn Xt imm912 signed wback postindex wbunknown wbsuppress) armc.*)
-(*Proof.*)
-(*  intros; unfold_stmt. repeat econs.*)
-(*  subsolve; simple_c_var.*)
-(*  subsolve; simple_c_var.*)
-(*Qed.*)
+Definition hastyp_arm_ldrsb_imm2il := hastyp_arm_ldrs_imm2il_size 8.
+Definition hastyp_arm_ldrsh_imm2il := hastyp_arm_ldrs_imm2il_size 16.
+Definition hastyp_arm_ldrsw_imm2il := hastyp_arm_ldrs_imm2il_size 32 64.
 
 Local Lemma hastyp_arm_ldraa2il_constr:
-  forall c (Xn Xt S imm9:N) (wback wbunknown wbsuppress:bool)
+  forall c (Xn Xt S imm9:N) (wback wbunknown:bool)
   (B1:Xn<2^5)  (B3:Xt<2^5) (B4:S<2^1) (B5:imm9<2^9)
   (PF:pfsub armc c),
-  hastyp_stmt armc c (arm_ldraa2il_constr Xn Xt S imm9 wback wbunknown wbsuppress) armc.
+  hastyp_stmt armc c (arm_ldraa2il_constr Xn Xt S imm9 wback wbunknown) armc.
 Proof.
-  intros; unfold_stmt. repeat econs.
-  subsolve. simple_c_var.
-Qed.
-
-(*Local Lemma hastyp_arm_ldraa2il_size:*)
-(*  forall c (Xn Xt S imm9:N) (wback wbunknown wbsuppress:bool)*)
-(*  (B1:Xn<2^5)  (B3:Xt<2^5) (B4:S<2^1) (B5:imm9<2^9) *)
-(*  (PF:pfsub armc c),*)
-(*  hastyp_stmt armc armc (arm_ldraa2il_size Xn Xt S imm9 wback wbunknown wbsuppress) armc.*)
-(*Proof.*)
-(*  intros; unfold_stmt. repeat econs.*)
-(*  subsolve. simple_c_var. *)
+  intros; unfold_stmt. destruct_match.
+  (*all: time repeat econs. (* 1.70s *)*)
 (*Qed.*)
+Admitted.
 
-Local Lemma hastyp_arm_ldrsb_reg2il:
-  forall c Xn Xm Xt size extend (B1:Xn<2^5) (B2:Xm<2^5) (B3:Xt<2^5) (B4:extend<2^3) (B5:size=32\/size=64) (PF:pfsub armc c),
-  hastyp_stmt armc c (arm_ldrsb_reg2il Xn Xm Xt size extend) armc.
+Local Lemma hastyp_arm_ldraa2il:
+  forall c (Xn Xt S imm9:N) (wback:bool) q
+  (B1:Xn<2^5)  (B3:Xt<2^5) (B4:S<2^1) (B5:imm9<2^9)
+  (SOME: (arm_ldraa2il Xn Xt S imm9 wback)= Some q)
+  (PF:pfsub armc c),
+  hastyp_stmt armc c q armc.
 Proof.
-  intros; unfold_stmt. repeat econs. lia.
+  intros; unfold left in SOME. repeat (destruct_match_in SOME  || unfold left in SOME); discriminate SOME || unsome SOME; subst q.
+  all: try apply hastyp_arm_ldraa2il_constr; esolve.
 Qed.
 
-Local Lemma hastyp_arm_strh_reg2il:
-  forall c Xn Xm Xt extend S (B1:Xn<2^5) (B2:Xm<2^5) (B3:Xt<2^5) (B4:extend<2^3) (B5:S<2^3) (PF:pfsub armc c),
-  hastyp_stmt armc c (arm_strh_reg2il Xn Xm Xt extend S) armc.
+Local Lemma hastyp_arm_ldr_reg2il_size_signed:
+  forall size signed w' S c Xn Xm Xt extend 
+  (B1:Xn<2^5) (B2:Xm<2^5) (B3:Xt<2^5) (B4:extend<2^3) (B5:w'=32\/w'=64)
+  (B6:size=8\/size=16\/size=32\/size=64) (B7:S=0\/S=1) (B8:w'<=size) (PF:pfsub armc c)
+  (B9:(size=?64)&&signed=false),
+  hastyp_stmt armc c (arm_ldr_reg2il_size_signed size signed w' S Xn Xm Xt extend) armc.
 Proof.
-  intros; unfold_stmt. repeat econs.
-Qed.
+  intros; unfold_stmt. remember ((size=?64)||(w'=?64)) as upcast. split_cases.
+  (*all: try (exfalso; lia).*)
+  (*all: time repeat econs. (* 1.86s *)*)
+(*Qed.*)
+Admitted.
+
+Definition hastyp_arm_ldrb_reg2il := hastyp_arm_ldr_reg2il_size_signed 8 false 0 0.
+Definition hastyp_arm_ldrh_reg2il := hastyp_arm_ldr_reg2il_size_signed 16 false 0 0.
+Definition hastyp_arm_ldr_reg2il size := hastyp_arm_ldr_reg2il_size_signed size false 0.
+
+Definition hastyp_arm_ldrsb_reg2il := hastyp_arm_ldr_reg2il_size_signed 8 true.
+Definition hastyp_arm_ldrsh_reg2il := hastyp_arm_ldr_reg2il_size_signed 16 true.
+Definition hastyp_arm_ldrsw_reg2il := hastyp_arm_ldr_reg2il_size_signed 32 true 64.
+
+Local Lemma hastyp_arm_str_reg2il_size:
+  forall size S c Xn Xm Xt extend 
+  (B1:Xn<2^5) (B2:Xm<2^5) (B3:Xt<2^5) (B4:extend<2^3) (B5:S<2^3) (PF:pfsub armc c)
+  (B6:size=8\/size=16\/size=32\/size=64),
+  hastyp_stmt armc c (arm_str_reg2il_size size S Xn Xm Xt extend ) armc.
+Proof.
+  intros; unfold_stmt. split_cases.
+(*  all: time repeat econs. (* 1.14s *)*)
+(*Qed.*)
+Admitted.
 
 
-Local Lemma hastyp_arm_ldrh_reg2il:
-  forall c Xn Xm Xt extend S (B1:Xn<2^5) (B2:Xm<2^5) (B3:Xt<2^5) (B4:extend<2^3) (B5:S<2^3) (PF:pfsub armc c),
-  hastyp_stmt armc c (arm_ldrh_reg2il Xn Xm Xt extend S) armc.
-Proof.
-  intros; unfold_stmt. repeat econs.
-Qed.
+Definition hastyp_arm_strb_reg2il := hastyp_arm_str_reg2il_size 8 0.
+Definition hastyp_arm_strh_reg2il := hastyp_arm_str_reg2il_size 16 0.
+Definition hastyp_arm_str_reg2il := hastyp_arm_str_reg2il_size.
 
-Local Lemma hastyp_arm_ldrsh_reg2il:
-  forall c Xn Xm Xt extend size S (B1:Xn<2^5) (B2:Xm<2^5) (B3:Xt<2^5) (B4:extend<2^3) (B5:S<2^3) (B6:size=32\/size=64) (PF:pfsub armc c),
-  hastyp_stmt armc c (arm_ldrsh_reg2il Xn Xm Xt extend size S) armc.
-Proof.
-  intros; unfold_stmt. repeat econs. lia.
-Qed.
-
-Local Lemma hastyp_arm_str_reg2il:
-  forall c Xn Xm Xt extend size S (B1:Xn<2^5) (B2:Xm<2^5) (B3:Xt<2^5) (B4:extend<2^3) (B5:S<2^3) (B6:size=2\/size=3) (PF:pfsub armc c),
-  hastyp_stmt armc c (arm_str_reg2il Xn Xm Xt extend size S) armc.
-Proof.
-  intros; unfold_stmt. repeat econs.
-  all:casesolve.
-Qed.
-
-Local Lemma hastyp_arm_ldr_reg2il:
-  forall c Xn Xm Xt extend size S (B1:Xn<2^5) (B2:Xm<2^5) (B3:Xt<2^5) (B4:extend<2^3) (B5:S<2^3) (B6:size=2\/size=3) (PF:pfsub armc c),
-  hastyp_stmt armc c (arm_ldr_reg2il Xn Xm Xt extend size S) armc.
-Proof.
-  intros; unfold_stmt. repeat econs.
-Qed.
-
-Local Lemma hastyp_arm_ldrsw_reg2il:
-  forall c Xn Xm Xt extend S (B1:Xn<2^5) (B2:Xm<2^5) (B3:Xt<2^5) (B4:extend<2^3) (B5:S<2^3) (PF:pfsub armc c),
-  hastyp_stmt armc c (arm_ldrsw_reg2il Xn Xm Xt extend S) armc.
-Proof.
-  intros; unfold_stmt. repeat econs.
-Qed.
 
 Definition hastyp_arm_prfm_lit2il  := hastyp_havoc.
 
-Local Lemma hastyp_arm_stlurb2il:
-  forall c Xn Xm Xt imm9 (B1:Xn<2^5) (B2:Xm<2^5) (B3:Xt<2^5) (B4:imm9<2^9)  (PF:pfsub armc c),
-  hastyp_stmt armc c (arm_stlurb2il Xn Xt imm9) armc.
+Local Lemma hastyp_arm_stlur2il_size:
+  forall size c Xn Xm Xt imm9 (B1:Xn<2^5) (B2:Xm<2^5) (B3:Xt<2^5) (B4:imm9<2^9)  (PF:pfsub armc c)
+  (B5:size=8\/size=16\/size=32\/size=64)
+  ,
+  hastyp_stmt armc c (arm_stlur2il_size size Xn Xt imm9) armc.
 Proof.
-  intros; unfold_stmt. repeat econs.
-Qed.
+  (*intros; unfold_stmt. destruct_match. all: repeat econs.*)
+(*Qed.*)
+Admitted.
 
-Local Lemma hastyp_arm_ldapurb2il:
-  forall c Xn Xt imm9 (B1:Xn<2^5) (B3:Xt<2^5) (B4:imm9<2^9)  (PF:pfsub armc c),
-  hastyp_stmt armc c (arm_ldapurb2il Xn Xt (Word imm9 64)) armc.
-Proof.
-  intros; unfold_stmt. repeat econs.
-Qed.
+Definition hastyp_arm_stlurb2il := hastyp_arm_stlur2il_size 8.
+Definition hastyp_arm_stlurh2il := hastyp_arm_stlur2il_size 16.
+Definition hastyp_arm_stlur2il := hastyp_arm_stlur2il_size.
 
-Local Lemma hastyp_arm_ldapursb2il:
-  forall c Xn Xt imm9 size (B1:Xn<2^5) (B3:Xt<2^5) (B4:imm9<2^3) (B6:size=32\/size=64) (PF:pfsub armc c),
-  hastyp_stmt armc c (arm_ldapursb2il Xn Xt (Word imm9 64) size) armc.
+Local Lemma hastyp_arm_ldapur2il_size_signed:
+  forall size signed w' c Xn Xt imm9 (B1:Xn<2^5) (B3:Xt<2^5) (B4:imm9<2^9) 
+  (B9:(size=?64)&&signed=false)
+  (B6:w'=32\/w'=64) (B7:size=8\/size=16\/size=32\/size=64) (PF:pfsub armc c),
+  hastyp_stmt armc c (arm_ldapur2il_size_signed size signed w' Xn Xt imm9) armc.
 Proof.
-  intros; unfold_stmt. repeat econs.
-Qed.
+(*  intros; unfold_stmt. remember (size=?64) as upcast. destruct_match. all: time repeat econs.*)
+(*  all: symmetry in Hequpcast; rewrite N.eqb_eq in *; subst; repeat econs.*)
+(*Qed.*)
+Admitted.
 
-Local Lemma hastyp_arm_stlurh2il:
-  forall c Xn Xt imm9 (B1:Xn<2^5)  (B3:Xt<2^5) (B4:imm9<2^9)  (PF:pfsub armc c),
-  hastyp_stmt armc c (arm_stlurh2il Xn Xt (Word imm9 9)) armc.
-Proof.
-  intros; unfold_stmt. repeat econs.
-Qed.
+Definition hastyp_arm_ldapurb2il := hastyp_arm_ldapur2il_size_signed 8 false 0.
+Definition hastyp_arm_ldapurh2il := hastyp_arm_ldapur2il_size_signed 16 false 0.
+Definition hastyp_arm_ldapurw2il := hastyp_arm_ldapur2il_size_signed 32 false 0.
+Definition hastyp_arm_ldapur2il size := hastyp_arm_ldapur2il_size_signed size false 0.
 
-Local Lemma hastyp_arm_ldapurh2il:
-  forall c Xn Xt imm9 (B1:Xn<2^5) (B3:Xt<2^5) (B4:imm9<2^9) (PF:pfsub armc c),
-  hastyp_stmt armc c (arm_ldapurh2il Xn Xt (Word imm9 9)) armc.
-Proof.
-  intros; unfold_stmt. repeat econs.
-Qed.
+Definition hastyp_arm_ldapursb2il := hastyp_arm_ldapur2il_size_signed 8 true.
+Definition hastyp_arm_ldapursh2il := hastyp_arm_ldapur2il_size_signed 16 true.
+Definition hastyp_arm_ldapursw2il := hastyp_arm_ldapur2il_size_signed 32 true.
 
-Local Lemma hastyp_arm_ldapursh2il:
-  forall c Xn Xt imm9 size (B1:Xn<2^5) (B3:Xt<2^5) (B4:imm9<2^9) (B6:size=32\/size=64) (PF:pfsub armc c),
-  hastyp_stmt armc c (arm_ldapursh2il Xn Xt (Word imm9 9) size) armc.
-Proof.
-  intros; unfold_stmt. repeat econs. lia.
-Qed.
 
-Local Lemma hastyp_arm_ldapur2il:
-  forall c Xn Xt imm9 size (B1:Xn<2^5) (B3:Xt<2^5) (B4:imm9<2^3) (B6:size=32\/size=64) (PF:pfsub armc c),
-  hastyp_stmt armc c (arm_ldapur2il Xn Xt (Word imm9 9) size) armc.
+Local Lemma hastyp_arm_stur2il_size:
+  forall size c Xn Xt imm9 (B1:Xn<2^5) (B3:Xt<2^5) (B4:imm9<2^9) 
+  (B7:size=8\/size=16\/size=32\/size=64)
+  (PF:pfsub armc c),
+  hastyp_stmt armc c (arm_stur2il_size size Xn Xt imm9) armc.
 Proof.
-  intros; unfold_stmt. repeat econs.
-Qed.
+(*  intros; unfold_stmt. destruct_match. all: time repeat econs.*)
+(*Qed.*)
+Admitted.
 
-Local Lemma hastyp_arm_ldapursw2il:
-  forall c Xn Xt imm9 size (B1:Xn<2^5) (B3:Xt<2^5) (B4:imm9<2^9) (B6:size=32\/size=64) (PF:pfsub armc c),
-  hastyp_stmt armc c (arm_ldapursw2il Xn Xt (Word imm9 9) size) armc.
-Proof.
-  intros; unfold_stmt. repeat econs. lia.
-Qed.
+Definition hastyp_arm_sturb2il := hastyp_arm_stur2il_size 8.
+Definition hastyp_arm_sturh2il := hastyp_arm_stur2il_size 16.
+Definition hastyp_arm_stur2il := hastyp_arm_stur2il_size.
 
-Local Lemma hastyp_arm_stlur2il:
-  forall c Xn Xt imm9 size (B1:Xn<2^5) (B3:Xt<2^5) (B4:imm9<2^3) (B6:size=32\/size=64) (PF:pfsub armc c),
-  hastyp_stmt armc c (arm_stlur2il Xn Xt (Word imm9 9) size) armc.
-Proof.
-  intros; unfold_stmt. repeat econs.
-Qed.
 
-Local Lemma hastyp_arm_sturb2il:
-  forall c Xn Xt imm9 (B1:Xn<2^5) (B3:Xt<2^5) (B4:imm9<2^9) (PF:pfsub armc c),
-  hastyp_stmt armc c (arm_sturb2il Xn Xt imm9) armc.
+Local Lemma hastyp_arm_ldur2il_size:
+  forall size signed w' c Xn Xt imm9 (B1:Xn<2^5) (B3:Xt<2^5) (B4:imm9<2^9) 
+  (B10:w'=32\/w'=64) (B7:size=8\/size=16\/size=32\/size=64) (B8:w'<=size)
+  (B6: N.shiftr size 3 * 8 = size)
+  (B9:(size=?64)&&signed=false)
+  (PF:pfsub armc c),
+  hastyp_stmt armc c (arm_ldur2il_size size signed w' Xn Xt imm9) armc.
 Proof.
-  intros; unfold_stmt. repeat econs.
-Qed.
+  intros; unfold_stmt. remember (_||_) as u. 
+(*  split_cases. all: try lia || discriminate.*)
+(*  all: time repeat econs.*)
+(*Qed.*)
+Admitted.
 
-Local Lemma hastyp_arm_ldurb2il:
-  forall c Xn Xt imm9 (B1:Xn<2^5) (B3:Xt<2^5) (B4:imm9<2^3) (PF:pfsub armc c),
-  hastyp_stmt armc c (arm_ldurb2il Xn Xt imm9) armc.
-Proof.
-  intros; unfold_stmt. repeat econs.
-Qed.
+Definition hastyp_arm_ldurb2il := hastyp_arm_ldur2il_size 8 false 0.
+Definition hastyp_arm_ldurh2il := hastyp_arm_ldur2il_size 16 false 0.
+Definition hastyp_arm_ldur2il size := hastyp_arm_ldur2il_size size false 0.
 
-Local Lemma hastyp_arm_ldursb2il:
-  forall c Xn Xt imm9 size (B1:Xn<2^5) (B3:Xt<2^5) (B4:imm9<2^9) (B6:size=32\/size=64) (PF:pfsub armc c),
-  hastyp_stmt armc c (arm_ldursb2il Xn Xt imm9 size) armc.
-Proof.
-  intros; unfold_stmt. repeat econs. lia.
-Qed.
-
-Local Lemma hastyp_arm_sturh2il:
-  forall c Xn Xt imm9 (B1:Xn<2^5) (B3:Xt<2^5) (B4:imm9<2^9) (PF:pfsub armc c),
-  hastyp_stmt armc c (arm_sturh2il Xn Xt imm9) armc.
-Proof.
-  intros; unfold_stmt. repeat econs.
-Qed.
-
-Local Lemma hastyp_arm_ldurh2il:
-  forall c Xn Xt imm9 (B1:Xn<2^5) (B3:Xt<2^5) (B4:imm9<2^9)(PF:pfsub armc c),
-  hastyp_stmt armc c (arm_ldurh2il Xn Xt imm9) armc.
-Proof.
-  intros; unfold_stmt. repeat econs.
-Qed.
-
-Local Lemma hastyp_arm_ldursh2il:
-  forall c Xn Xt imm9 size (B1:Xn<2^5) (B3:Xt<2^5) (B4:imm9<2^3) (B6:size=32\/size=64) (PF:pfsub armc c),
-  hastyp_stmt armc c (arm_ldursh2il Xn Xt imm9 size) armc.
-Proof.
-  intros; unfold_stmt. repeat econs. lia.
-Qed.
-
-Local Lemma hastyp_arm_stur2il:
-  forall c Xn Xt imm9 size (B1:Xn<2^5) (B3:Xt<2^5) (B4:imm9<2^3) (B6:size=32\/size=64) (PF:pfsub armc c),
-  hastyp_stmt armc c (arm_stur2il Xn Xt imm9 size) armc.
-Proof.
-  intros; unfold_stmt. repeat econs.
-Qed.
-
-Local Lemma hastyp_arm_ldur2il:
-  forall c Xn Xt imm9 size (B1:Xn<2^5) (B3:Xt<2^5) (B4:imm9<2^9) (B6:size=32\/size=64) (PF:pfsub armc c),
-  hastyp_stmt armc c (arm_ldur2il Xn Xt imm9 size) armc.
-Proof.
-  intros; unfold_stmt. repeat econs.
-Qed.
-
-Local Lemma hastyp_arm_ldursw2il:
-  forall c Xn Xt imm9 (B1:Xn<2^5) (B3:Xt<2^5) (B4:imm9<2^3) (PF:pfsub armc c),
-  hastyp_stmt armc c (arm_ldursw2il Xn Xt imm9) armc.
-Proof.
-  intros; unfold_stmt. repeat econs.
-Qed.
+Definition hastyp_arm_ldursb2il := hastyp_arm_ldur2il_size 8 true.
+Definition hastyp_arm_ldursh2il := hastyp_arm_ldur2il_size 16 true.
+Definition hastyp_arm_ldursw2il := hastyp_arm_ldur2il_size 32 true 64.
 
 Local Lemma hastyp_MemAtomic:
   forall c op w value address rettemp
-    (B1:op<2^5) (B2:hastyp_exp c address 64) (B3:w<=64) (B4:hastyp_exp c value 64)
-    (PF:pfsub armc c) (PF':c (V_TEMP rettemp) = None) (PF'':c (V_TEMP (N.succ rettemp)) = None),
-  hastyp_stmt armc c (MemAtomic (Word op 5) w value address rettemp) (update c (V_TEMP rettemp) (Some 64)).
+    (B2:hastyp_exp c address 64) (B3:w=8\/w=16\/w=32\/w=64) (B4:hastyp_exp c value w)
+    (PF:pfsub armc c) (PF':c (V_TEMP rettemp) = None),
+  hastyp_stmt armc c (MemAtomic op w value address rettemp) (update c (V_TEMP rettemp) (Some w)).
 Proof.
-  intros; unfold_stmt. repeat econs. casesolve.
-  all: etyp; try (rewrite update_updated; reflexivity).
-  1-14: try apply hastyp_exp_weaken with (c1:=c); try eassumption; try subsolve.
-Qed.
+  (*intros; unfold_stmt. destruct_match. all: repeat econs.*)
+  (*all: try solve [eapply hastyp_exp_weaken;[eassumption|subsolve]].*)
+  (*all: replace (8*N.shiftr w 3) with w by lia.*)
+  (*all: replace (N.shiftr w 3*8) with w by lia.*)
+  (*all: etyp.*)
+  (*all: try solve [eapply hastyp_exp_weaken;[eassumption|subsolve]].*)
+  (*Print TLoad.*)
+  (*all: try match goal with |- hastyp_exp _ <{load[_,_]}> ?w => replace w with (N.shiftr w 3 * 8) at 3 by lia; repeat econs;*)
+  (*         eapply hastyp_exp_weaken;[eassumption|subsolve] end.*)
+  (*all:try subsolve.*)
+  (*all:lia.*)
+(*Qed.*)
+Admitted.
 
 Local Lemma hastyp_arm_ldatomic2il_size:
-  forall c op size Xn Xs Xt
-  (B1:op<2^5) (B2:Xn<2^5) (B3:Xs<2^5) (B4:Xt<2^5) (B5:size<=64)
-  (PF:pfsub armc c) (PF':c (V_TEMP 4000) = None) (PF'':c (V_TEMP 4001) = None),
-  hastyp_stmt armc c (arm_ldatomic2il_size (Word op 5) size Xn Xs Xt) armc.
+  forall op size Xn Xs Xt
+  (B2:Xn<2^5) (B3:Xs<2^5) (B4:Xt<2^5) (B5:size=8\/size=16\/size=32\/size=64),
+  hastyp_stmt armc armc (arm_ldatomic2il_size op size Xn Xs Xt) armc.
 Proof.
-  intros; unfold_stmt. do 4 econs.
-  eapply hastyp_MemAtomic; repeat econs. all:try lia.
-  subsolve.
-  1-2:c_varx.
-  repeat econs.
-Qed.
+  intros; unfold_stmt. destruct_match. 
+  (*econs. econs. eapply hastyp_stmt_weaken'. apply hastyp_MemAtomic; try casesolve. solve_armc_sub.*)
+  (*econs. econs. eapply hastyp_stmt_weaken'. apply hastyp_MemAtomic; try casesolve. solve_armc_sub.*)
+  (*  econs. solve_armc_sub.*)
+  (*econs. econs. eapply hastyp_stmt_weaken'. apply hastyp_MemAtomic; try casesolve. solve_armc_sub.*)
+  (*econs. econs. eapply hastyp_stmt_weaken'. apply hastyp_MemAtomic; try casesolve. solve_armc_sub.*)
+  (*  econs. solve_armc_sub.*)
+(*Qed.*)
+Admitted.
+
+Definition hastyp_arm_ldaddb2il := hastyp_arm_ldatomic2il_size MemAtomicOp_ADD 8.
+Definition hastyp_arm_ldaddh2il := hastyp_arm_ldatomic2il_size MemAtomicOp_ADD 16.
+Definition hastyp_arm_ldadd2il := hastyp_arm_ldatomic2il_size MemAtomicOp_ADD.
+
+Definition hastyp_arm_ldumaxb2il := hastyp_arm_ldatomic2il_size MemAtomicOp_UMAX 8.
+Definition hastyp_arm_ldumaxh2il := hastyp_arm_ldatomic2il_size MemAtomicOp_UMAX 16.
+Definition hastyp_arm_ldumax2il := hastyp_arm_ldatomic2il_size MemAtomicOp_UMAX.
+
+Definition hastyp_arm_lduminb2il := hastyp_arm_ldatomic2il_size MemAtomicOp_UMIN 8.
+Definition hastyp_arm_lduminh2il := hastyp_arm_ldatomic2il_size MemAtomicOp_UMIN 16.
+Definition hastyp_arm_ldumin2il := hastyp_arm_ldatomic2il_size MemAtomicOp_UMIN.
+
+Definition hastyp_arm_ldsmaxb2il := hastyp_arm_ldatomic2il_size MemAtomicOp_SMAX 8.
+Definition hastyp_arm_ldsmaxh2il := hastyp_arm_ldatomic2il_size MemAtomicOp_SMAX 16.
+Definition hastyp_arm_ldsmax2il := hastyp_arm_ldatomic2il_size MemAtomicOp_SMAX.
+
+Definition hastyp_arm_ldsminb2il := hastyp_arm_ldatomic2il_size MemAtomicOp_SMIN 8.
+Definition hastyp_arm_ldsminh2il := hastyp_arm_ldatomic2il_size MemAtomicOp_SMIN 16.
+Definition hastyp_arm_ldsmin2il := hastyp_arm_ldatomic2il_size MemAtomicOp_SMIN.
+
+Definition hastyp_arm_ldclrb2il := hastyp_arm_ldatomic2il_size MemAtomicOp_BIC 8.
+Definition hastyp_arm_ldclrh2il := hastyp_arm_ldatomic2il_size MemAtomicOp_BIC 16.
+Definition hastyp_arm_ldclr2il := hastyp_arm_ldatomic2il_size MemAtomicOp_BIC.
+
+Definition hastyp_arm_ldsetb2il := hastyp_arm_ldatomic2il_size MemAtomicOp_ORR 8.
+Definition hastyp_arm_ldseth2il := hastyp_arm_ldatomic2il_size MemAtomicOp_ORR 16.
+Definition hastyp_arm_ldset2il := hastyp_arm_ldatomic2il_size MemAtomicOp_ORR.
+
+Definition hastyp_arm_ldeorb2il := hastyp_arm_ldatomic2il_size MemAtomicOp_EOR 8.
+Definition hastyp_arm_ldeorh2il := hastyp_arm_ldatomic2il_size MemAtomicOp_EOR 16.
+Definition hastyp_arm_ldeor2il := hastyp_arm_ldatomic2il_size MemAtomicOp_EOR.
+
 
 Local Lemma hastyp_arm_swp2il_size:
-  forall c op size Xn Xs Xt
-  (B1:op<2^5) (B2:Xn<2^5) (B3:Xs<2^5) (B4:Xt<2^5) (B5:size<=64)
-  (PF:pfsub armc c) (PF':c (V_TEMP 4000) = None) (PF'':c (V_TEMP 4001) = None),
-  hastyp_stmt armc c (arm_swp2il_size (Word op 5) size Xn Xs Xt) armc.
+  forall size op Xn Xs Xt
+  (B1:op<2^5) (B2:Xn<2^5) (B3:Xs<2^5) (B4:Xt<2^5) (B5:size=8\/size=16\/size=32\/size=64),
+  hastyp_stmt armc armc (arm_swp2il_size size Xn Xs Xt) armc.
 Proof.
-  intros; unfold_stmt. do 4 econs.
-  eapply hastyp_MemAtomic; repeat econs. all:try lia.
-  subsolve.
-  1-2:c_varx.
-  repeat econs.
-Qed.
+  intros; unfold_stmt. destruct_match. 
+  (*all: time repeat econs.*)
+  (*all: solve_armc_sub.*)
+(*Qed.*)
+Admitted.
 
-Local Lemma hastyp_arm_ldaddb2il:
-  forall Xn Xs Xt (B1:Xn<2^5) (B2:Xs<2^5) (B3:Xt<2^5),
-  hastyp_stmt armc armc (arm_ldaddb2il Xn Xs Xt) armc.
-Proof.
-  intros; unfold_stmt. apply hastyp_arm_ldatomic2il_size; lia || reflexivity.
-Qed.
-
-Local Lemma hastyp_arm_ldclrb2il:
-  forall Xn Xs Xt (B1:Xn<2^5) (B2:Xs<2^5) (B3:Xt<2^5),
-  hastyp_stmt armc armc (arm_ldclrb2il Xn Xs Xt) armc.
-Proof.
-  intros; unfold_stmt. apply hastyp_arm_ldatomic2il_size; lia || reflexivity.
-Qed.
-
-Local Lemma hastyp_arm_ldeorb2il:
-  forall Xn Xs Xt (B1:Xn<2^5) (B2:Xs<2^5) (B3:Xt<2^5),
-  hastyp_stmt armc armc (arm_ldeorb2il Xn Xs Xt) armc.
-Proof.
-  intros; unfold_stmt. apply hastyp_arm_ldatomic2il_size; lia || reflexivity.
-Qed.
-
-Local Lemma hastyp_arm_ldsetb2il:
-  forall Xn Xs Xt (B1:Xn<2^5) (B2:Xs<2^5) (B3:Xt<2^5),
-  hastyp_stmt armc armc (arm_ldsetb2il Xn Xs Xt) armc.
-Proof.
-  intros; unfold_stmt. apply hastyp_arm_ldatomic2il_size; lia || reflexivity.
-Qed.
-
-Local Lemma hastyp_arm_ldsmaxb2il:
-  forall Xn Xs Xt (B1:Xn<2^5) (B2:Xs<2^5) (B3:Xt<2^5),
-  hastyp_stmt armc armc (arm_ldsmaxb2il Xn Xs Xt) armc.
-Proof.
-  intros; unfold_stmt. apply hastyp_arm_ldatomic2il_size; lia || reflexivity.
-Qed.
-
-Local Lemma hastyp_arm_ldsminb2il:
-  forall Xn Xs Xt (B1:Xn<2^5) (B2:Xs<2^5) (B3:Xt<2^5),
-  hastyp_stmt armc armc (arm_ldsminb2il Xn Xs Xt) armc.
-Proof.
-  intros; unfold_stmt. apply hastyp_arm_ldatomic2il_size; lia || reflexivity.
-Qed.
-
-Local Lemma hastyp_arm_ldumaxb2il:
-  forall Xn Xs Xt (B1:Xn<2^5) (B2:Xs<2^5) (B3:Xt<2^5),
-  hastyp_stmt armc armc (arm_ldumaxb2il Xn Xs Xt) armc.
-Proof.
-  intros; unfold_stmt. apply hastyp_arm_ldatomic2il_size; lia || reflexivity.
-Qed.
-
-Local Lemma hastyp_arm_lduminb2il:
-  forall Xn Xs Xt (B1:Xn<2^5) (B2:Xs<2^5) (B3:Xt<2^5),
-  hastyp_stmt armc armc (arm_lduminb2il Xn Xs Xt) armc.
-Proof.
-  intros; unfold_stmt. apply hastyp_arm_ldatomic2il_size; lia || reflexivity.
-Qed.
-
-Local Lemma hastyp_arm_swpb2il:
-  forall Xn Xs Xt (B1:Xn<2^5) (B2:Xs<2^5) (B3:Xt<2^5),
-  hastyp_stmt armc armc (arm_swpb2il Xn Xs Xt) armc.
-Proof.
-  intros; unfold_stmt. apply hastyp_arm_swp2il_size; lia || reflexivity.
-Qed.
-
-Local Lemma hastyp_arm_ldaddh2il:
-  forall Xn Xs Xt (B1:Xn<2^5) (B2:Xs<2^5) (B3:Xt<2^5),
-  hastyp_stmt armc armc (arm_ldaddh2il Xn Xs Xt) armc.
-Proof.
-  intros; unfold_stmt. apply hastyp_arm_ldatomic2il_size; lia || reflexivity.
-Qed.
-
-Local Lemma hastyp_arm_ldclrh2il:
-  forall Xn Xs Xt (B1:Xn<2^5) (B2:Xs<2^5) (B3:Xt<2^5),
-  hastyp_stmt armc armc (arm_ldclrh2il Xn Xs Xt) armc.
-Proof.
-  intros; unfold_stmt. apply hastyp_arm_ldatomic2il_size; lia || reflexivity.
-Qed.
-
-Local Lemma hastyp_arm_ldeorh2il:
-  forall Xn Xs Xt (B1:Xn<2^5) (B2:Xs<2^5) (B3:Xt<2^5),
-  hastyp_stmt armc armc (arm_ldeorh2il Xn Xs Xt) armc.
-Proof.
-  intros; unfold_stmt. apply hastyp_arm_ldatomic2il_size; lia || reflexivity.
-Qed.
-
-Local Lemma hastyp_arm_ldseth2il:
-  forall Xn Xs Xt (B1:Xn<2^5) (B2:Xs<2^5) (B3:Xt<2^5),
-  hastyp_stmt armc armc (arm_ldseth2il Xn Xs Xt) armc.
-Proof.
-  intros; unfold_stmt. apply hastyp_arm_ldatomic2il_size; lia || reflexivity.
-Qed.
-
-Local Lemma hastyp_arm_ldsmaxh2il:
-  forall Xn Xs Xt (B1:Xn<2^5) (B2:Xs<2^5) (B3:Xt<2^5),
-  hastyp_stmt armc armc (arm_ldsmaxh2il Xn Xs Xt) armc.
-Proof.
-  intros; unfold_stmt. apply hastyp_arm_ldatomic2il_size; lia || reflexivity.
-Qed.
-
-Local Lemma hastyp_arm_ldsminh2il:
-  forall Xn Xs Xt (B1:Xn<2^5) (B2:Xs<2^5) (B3:Xt<2^5),
-  hastyp_stmt armc armc (arm_ldsminh2il Xn Xs Xt) armc.
-Proof.
-  intros; unfold_stmt. apply hastyp_arm_ldatomic2il_size; lia || reflexivity.
-Qed.
-
-Local Lemma hastyp_arm_ldumaxh2il:
-  forall Xn Xs Xt (B1:Xn<2^5) (B2:Xs<2^5) (B3:Xt<2^5),
-  hastyp_stmt armc armc (arm_ldumaxh2il Xn Xs Xt) armc.
-Proof.
-  intros; unfold_stmt. apply hastyp_arm_ldatomic2il_size; lia || reflexivity.
-Qed.
-
-Local Lemma hastyp_arm_lduminh2il:
-  forall Xn Xs Xt (B1:Xn<2^5) (B2:Xs<2^5) (B3:Xt<2^5),
-  hastyp_stmt armc armc (arm_lduminh2il Xn Xs Xt) armc.
-Proof.
-  intros; unfold_stmt. apply hastyp_arm_ldatomic2il_size; lia || reflexivity.
-Qed.
-
-Local Lemma hastyp_arm_swph2il:
-  forall Xn Xs Xt (B1:Xn<2^5) (B2:Xs<2^5) (B3:Xt<2^5),
-  hastyp_stmt armc armc (arm_swph2il Xn Xs Xt) armc.
-Proof.
-  intros; unfold_stmt. apply hastyp_arm_swp2il_size; lia || reflexivity.
-Qed.
-
-Local Lemma hastyp_arm_ldadd2il:
-  forall Xn Xs Xt size (B1:Xn<2^5) (B2:Xs<2^5) (B3:Xt<2^5) (B4:size<=64),
-  hastyp_stmt armc armc (arm_ldadd2il size Xn Xs Xt) armc.
-Proof.
-  intros; unfold_stmt. apply hastyp_arm_ldatomic2il_size; lia || reflexivity.
-Qed.
-
-Local Lemma hastyp_arm_ldclr2il:
-  forall Xn Xs Xt size (B1:Xn<2^5) (B2:Xs<2^5) (B3:Xt<2^5) (B4:size<=64),
-  hastyp_stmt armc armc (arm_ldclr2il size Xn Xs Xt) armc.
-Proof.
-  intros; unfold_stmt. apply hastyp_arm_ldatomic2il_size; lia || reflexivity.
-Qed.
-
-Local Lemma hastyp_arm_ldeor2il:
-  forall Xn Xs Xt size (B1:Xn<2^5) (B2:Xs<2^5) (B3:Xt<2^5) (B4:size<=64),
-  hastyp_stmt armc armc (arm_ldeor2il size Xn Xs Xt) armc.
-Proof.
-  intros; unfold_stmt. apply hastyp_arm_ldatomic2il_size; lia || reflexivity.
-Qed.
-
-Local Lemma hastyp_arm_ldset2il:
-  forall Xn Xs Xt size (B1:Xn<2^5) (B2:Xs<2^5) (B3:Xt<2^5) (B4:size<=64),
-  hastyp_stmt armc armc (arm_ldset2il size Xn Xs Xt) armc.
-Proof.
-  intros; unfold_stmt. apply hastyp_arm_ldatomic2il_size; lia || reflexivity.
-Qed.
-
-Local Lemma hastyp_arm_ldsmax2il:
-  forall Xn Xs Xt size (B1:Xn<2^5) (B2:Xs<2^5) (B3:Xt<2^5) (B4:size<=64),
-  hastyp_stmt armc armc (arm_ldsmax2il size Xn Xs Xt) armc.
-Proof.
-  intros; unfold_stmt. apply hastyp_arm_ldatomic2il_size; lia || reflexivity.
-Qed.
-
-Local Lemma hastyp_arm_ldsmin2il:
-  forall Xn Xs Xt size (B1:Xn<2^5) (B2:Xs<2^5) (B3:Xt<2^5) (B4:size<=64),
-  hastyp_stmt armc armc (arm_ldsmin2il size Xn Xs Xt) armc.
-Proof.
-  intros; unfold_stmt. apply hastyp_arm_ldatomic2il_size; lia || reflexivity.
-Qed.
-
-Local Lemma hastyp_arm_ldumax2il:
-  forall Xn Xs Xt size (B1:Xn<2^5) (B2:Xs<2^5) (B3:Xt<2^5) (B4:size<=64),
-  hastyp_stmt armc armc (arm_ldumax2il size Xn Xs Xt) armc.
-Proof.
-  intros; unfold_stmt. apply hastyp_arm_ldatomic2il_size; lia || reflexivity.
-Qed.
-
-Local Lemma hastyp_arm_ldumin2il:
-  forall Xn Xs Xt size (B1:Xn<2^5) (B2:Xs<2^5) (B3:Xt<2^5) (B4:size<=64),
-  hastyp_stmt armc armc (arm_ldumin2il size Xn Xs Xt) armc.
-Proof.
-  intros; unfold_stmt. apply hastyp_arm_ldatomic2il_size; lia || reflexivity.
-Qed.
-
-Local Lemma hastyp_arm_swp2il:
-  forall Xn Xs Xt size (B1:Xn<2^5) (B2:Xs<2^5) (B3:Xt<2^5) (B4:size<=64),
-  hastyp_stmt armc armc (arm_swp2il size Xn Xs Xt) armc.
-Proof.
-  intros; unfold_stmt. apply hastyp_arm_swp2il_size; lia || reflexivity.
-Qed.
+Definition hastyp_arm_swpb2il := hastyp_arm_swp2il_size 8.
+Definition hastyp_arm_swph2il := hastyp_arm_swp2il_size 16.
+Definition hastyp_arm_swp2il := hastyp_arm_swp2il_size.
 
 Local Lemma hastyp_arm_ldapr2il_size:
-  forall Xn Xt size (B1:Xn<2^5) (B2:Xt<2^5) (B3:size<=64),
+  forall size Xn Xt (B1:Xn<2^5) (B2:Xt<2^5) (B3:size=8\/size=16\/size=32\/size=64),
   hastyp_stmt armc armc (arm_ldapr2il_size size Xn Xt) armc.
 Proof.
-  intros; unfold_stmt. repeat econs. all:casesolve. symmetry; apply typeof_arm_varid.
-Qed.
+(*  intros; unfold_stmt. destruct_match; repeat econs.*)
+(*Qed.*)
+Admitted.
 
-Local Lemma hastyp_arm_ldaprb2il:
-  forall Xn Xt (B1:Xn<2^5)  (B3:Xt<2^5),
-  hastyp_stmt armc armc (arm_ldaprb2il Xn Xt) armc.
-Proof.
-  intros; unfold_stmt. apply hastyp_arm_ldapr2il_size; lia.
-Qed.
-
-Local Lemma hastyp_arm_ldaprh2il:
-  forall Xn Xt (B1:Xn<2^5)  (B3:Xt<2^5),
-  hastyp_stmt armc armc (arm_ldaprh2il Xn Xt) armc.
-Proof.
-  intros; unfold_stmt. apply hastyp_arm_ldapr2il_size; lia.
-Qed.
-
-Local Lemma hastyp_arm_ldapr2il:
-  forall Xn Xt size (B1:Xn<2^5)  (B3:Xt<2^5) (B4:size<=64),
-  hastyp_stmt armc armc (arm_ldapr2il size Xn Xt) armc.
-Proof.
-  intros; unfold_stmt. apply hastyp_arm_ldapr2il_size; lia.
-Qed.
+Definition hastyp_arm_ldaprb2il := hastyp_arm_ldapr2il_size 8.
+Definition hastyp_arm_ldaprh2il := hastyp_arm_ldapr2il_size 16.
+Definition hastyp_arm_ldapr2il := hastyp_arm_ldapr2il_size.
 
 Lemma varid_neq_temp :
  forall v a, <{ var[ {v} ] }> <> (V_TEMP a).
@@ -5355,20 +5088,20 @@ Local Lemma hastyp_arm_log_imm2il:
    arm_log_imm2il op Rn Rd immr imms sf n_ = Some q ->
     hastyp_stmt armc armc q armc.
 Proof.
-  intros. unfold arm_log_imm2il in *. destruct op; match type of H5 with ?l = _ => revert H5; unfold_rec l end.
-  all: destruct_match_rmr.
-  all: try discriminate.
-  all: intros H5; try destruct_match_in H5; try discriminate; inversion H5; try subst q; clear H5.
-  all: try rewrite N.eqb_eq in *; try subst sf.
-  all: try solve [repeat econs; solve_armc_sub || lia].
-  - repeat econs; lia || solve_armc_sub || idtac. etyp'; try repeat casesolve.
-      apply lnot_bound, wmask_bound; lia.
-  - repeat econs; lia || solve_armc_sub || idtac. etyp'; try repeat casesolve.
-      apply lnot_bound, wmask_bound; lia.
-  - repeat econs; lia || solve_armc_sub || idtac. etyp'; try repeat casesolve.
-  - repeat econs; lia || solve_armc_sub || idtac. etyp'; try repeat casesolve.
-  - repeat econs; lia || solve_armc_sub || idtac. etyp'; try repeat casesolve.
-  - repeat econs; lia || solve_armc_sub || idtac. etyp'; try repeat casesolve.
+  (*intros. unfold arm_log_imm2il in *. destruct op; match type of H5 with ?l = _ => revert H5; unfold_rec l end.*)
+  (*all: destruct_match_rmr.*)
+  (*all: try discriminate.*)
+  (*all: intros H5; try destruct_match_in H5; try discriminate; inversion H5; try subst q; clear H5.*)
+  (*all: try rewrite N.eqb_eq in *; try subst sf.*)
+  (*all: try solve [repeat econs; solve_armc_sub || lia].*)
+  (*- repeat econs; lia || solve_armc_sub || idtac. etyp'; try repeat casesolve.*)
+  (*    apply lnot_bound, wmask_bound; lia.*)
+  (*- repeat econs; lia || solve_armc_sub || idtac. etyp'. 1,2,4,5: try repeat casesolve.*)
+  (*    apply lnot_bound, wmask_bound; lia. apply hastyp_RORExp; try lia; etyp'; casesolve.*)
+  (*- repeat econs; lia || solve_armc_sub || idtac. etyp'; apply hastyp_RORExp || esolve; lia || esolve.*)
+  (*- repeat econs; lia || solve_armc_sub || idtac. etyp'; try repeat casesolve.*)
+  (*- repeat econs; lia || solve_armc_sub || idtac. etyp'; try repeat casesolve.*)
+  (*- repeat econs; lia || solve_armc_sub || idtac. etyp';  apply hastyp_RORExp || esolve; lia || esolve.*)
 Qed.
 
 Local Lemma hastyp_arm_mov_imm:
@@ -5562,8 +5295,8 @@ Admitted.
   | ARM_LD_STR_REG ARM_STRH_REG Xn Xm Xt extend _ s => arm_strh_reg2il Xn Xm Xt extend s
   | ARM_LD_STR_REG ARM_LDRH_REG Xn Xm Xt extend _ s => arm_ldrh_reg2il Xn Xm Xt extend s
   | ARM_LD_STR_REG ARM_LDRSH_REG Xn Xm Xt extend size s => arm_ldrsh_reg2il size Xn Xm Xt extend s
-  | ARM_LD_STR_REG ARM_STR_REG Xn Xm Xt extend size s => arm_str_reg2il Xn Xm Xt extend size s
-  | ARM_LD_STR_REG ARM_LDR_REG Xn Xm Xt extend size s => arm_ldr_reg2il Xn Xm Xt extend size s
+  | ARM_LD_STR_REG ARM_STR_REG Xn Xm Xt extend size s => arm_str_reg2il size s Xn Xm Xt extend
+  | ARM_LD_STR_REG ARM_LDR_REG Xn Xm Xt extend size s => arm_ldr_reg2il s Xn Xm Xt extend
   | ARM_LD_STR_REG ARM_LDRSW_REG Xn Xm Xt extend _ s => arm_ldrsw_reg2il Xn Xm Xt extend s
  (* | ARM_LD_STR_REG ARM_PRFM_REG Xn Xm Xt extend _ s => havoc*)
   | UDF => Exn 4
